Useful lemmas, mostly regarding memory
Co-authored-by: Jakub Kopański <jakub@famisoft.pl>

Clear/EVMState.lean
@@ -1,8 +1,16 @@
 import Mathlib.Data.Finmap
 import Mathlib.Data.Fin.Basic
+import Mathlib.Data.List.Intervals
 import Clear.Ast
 import Clear.Instr
 import Clear.UInt256
+import Clear.Wheels
+
+set_option linter.setOption false
+set_option pp.coercions false
+
+set_option maxHeartbeats 700000
+set_option maxRecDepth 800
 
 open Clear Instr UInt256
 
@@ -69,8 +77,10 @@ def Account.updateStorage (act : Account) (k v : UInt256) : Account :=
 
 -- definition of the machine state
 
+abbrev Memory := Finmap (λ _ : UInt256 ↦ UInt8)
+
 structure MachineState : Type where
-  memory        : Finmap (λ _ : UInt256 => UInt8)
+  memory        : Memory
   max_address   : UInt256
   gas_available : UInt256
   return_data   : List UInt256
@@ -80,28 +90,178 @@ instance : Inhabited MachineState := ⟨ MachineState.mk ∅ 0 0 [] ⟩
 
 -- @langfield: Nit, but definitions should be camelCase.
 
-def UInt256.offsets : List UInt256 :=
+def UInt256.offsets : List ℕ :=
   [0,1,2,3,4,5,6,7,8,9,10,11,12,13,14,15,16,
   17,18,19,20,21,22,23,24,25,26,27,28,29,30,31]
 
+lemma UInt256.offsets_def : offsets = List.range 32 := by
+  repeat rw [ List.range_succ_eq_map ]
+  unfold offsets
+  simp
+
+lemma max_of_offsets_lt_32 : offsets.maximum < 32 := by decide
+lemma min_of_offsets_eq_0 : offsets.minimum = 0 := by decide
+
+lemma mem_offsets : ∀ {n}, n ∈ offsets ↔ n < 32 := by
+  intro n
+  rw [offsets_def]
+  simp
+
+@[simp]
+lemma mem_offsets_of_lt_32 : ∀ {n}, n < 32 → n ∈ offsets :=
+  mem_offsets.mpr
+
+lemma lt_32_of_mem_offsets : ∀ {n}, n ∈ offsets → n < 32 :=
+  mem_offsets.mp
+
+-- List.Ico not yet in mathlib
+lemma UInt256.offsets_eq_Ico : offsets = List.Ico 0 32 := by
+  unfold List.Ico
+  rw [ List.range'_eq_map_range, offsets_def ]
+  simp
+
+-- lemma UInt256.offsets_at_addr :
+--   ∀ (addr : UInt256),
+--   offsets.map (addr + ↑·) = List.Ico addr.val (addr.val + 32) := by
+--   intro addr
+--   rw [offsets_eq_Ico, List.Ico.map_add 0 32 addr, zero_add, add_comm]
+
+lemma UInt256.mem_offsets_iff_mem_Ico : ∀ {n}, n ∈ offsets ↔ n ∈ Set.Ico 0 32 := by
+  intro n
+  apply Iff.intro
+  · intro mem
+    simp
+    exact mem_offsets.mp mem
+  · intro mem
+    simp at mem
+    exact mem_offsets.mpr mem
+
+lemma UInt256.offsetted_addresses (addr : UInt256) : ∀ {n},
+  (h : n ∈ offsets) → addr + ↑n ∈ offsets.map (addr + ↑·) := by
+  intro n h
+  exact List.mem_map_of_mem (addr + ↑·) h
+
+-- lemma UInt256.word_addresses (addr : UInt256) :
+--   Set.MapsTo (addr + ↑·) (Set.Ico 0 32) (Set.Ico addr (addr + 32)) := by
+--   have : (addr + ↑·) '' (Set.Ico 0 32) = Set.Ico addr (addr + 32) := by
+--     dsimp [Set.image]
+--     conv => rhs; rw [← Set.Ico_def]
+
+--     sorry
+
+--   rw [← this]
+--   exact Set.mapsTo_image (addr + ↑·) (Set.Ico 0 32)
+
+
+-- lemma UInt256.same_address_of_offsetted_addresses (addr addr': UInt256) {n} :
+--   (h : n ∈ offsets) →
+--   addr' + ↑n ∈ offsets.map (addr + ↑·) →
+--   addr' = addr := by
+--   intro h mem
+--   simp at mem
+--   sorry
+
+-- lemma UInt256.addresses_of (addr : UInt256) {a} :
+--   a ∈ offsets.map (addr + ↑·) ↔ a ∈ Set.Ico addr (addr + 32) := by
+--   sorry
+
+namespace UInt256
+
+def range' (start : UInt256) (len : ℕ) (step : UInt256 := 1) : List UInt256 :=
+  match start, len with
+  | _, 0 => []
+  | s, n + 1 => s :: range' (s + step) n step
+
+@[simp]
+lemma range'_zero {s step : UInt256} : range' s 0 step = [] := by
+  unfold range'
+  rfl
+
+@[simp]
+lemma range'_one {s step : UInt256} : range' s 1 step = [s] := by
+  unfold range'
+  simp
+
+lemma range'_succ (start : UInt256) (len : ℕ) (step : UInt256) :
+  range' start (len + 1) step =
+    start :: range' (start + step) len step := by
+  conv =>
+    lhs
+    unfold range'
+    simp
+
+-- lemma range'_succ' (start : UInt256) (len : ℕ) (step : UInt256) (k : ℕ) [NeZero k] :
+--   range' start (len + k) step =
+--     start :: range' (start + step) (len + k - 1) step := by
+--   admit
+
+lemma map_add_range' (a) : ∀ s n step,
+  List.map (a + ·) (range' s n step) =
+    range' (a + s) n step
+  | _, 0, _ => by simp
+  | s, n+1, step => by
+    unfold range'
+    simp [map_add_range', add_assoc]
+
+def offsets_at (addr : UInt256) : List UInt256 :=
+  range' addr 32 1
+
+def words_at (addr : UInt256) (n : ℕ) : List UInt256 :=
+  range' addr n 32
+
+end UInt256
+
+lemma splice_toBytes! (v : UInt256) : toBytes! v =
+  [ (toBytes! v)[0],   (toBytes! v)[1],   (toBytes! v)[2],   (toBytes! v)[3]
+  , (toBytes! v)[4],   (toBytes! v)[5],   (toBytes! v)[6],   (toBytes! v)[7]
+  , (toBytes! v)[8],   (toBytes! v)[9],   (toBytes! v)[10],  (toBytes! v)[11]
+  , (toBytes! v)[12],  (toBytes! v)[13],  (toBytes! v)[14],  (toBytes! v)[15]
+  , (toBytes! v)[16],  (toBytes! v)[17],  (toBytes! v)[18],  (toBytes! v)[19]
+  , (toBytes! v)[20],  (toBytes! v)[21],  (toBytes! v)[22],  (toBytes! v)[23]
+  , (toBytes! v)[24],  (toBytes! v)[25],  (toBytes! v)[26],  (toBytes! v)[27]
+  , (toBytes! v)[28],  (toBytes! v)[29],  (toBytes! v)[30],  (toBytes! v)[31]
+  ] := by
+  apply List.ext_get
+  · simp
+  · intro n h₁ h₂
+    simp at h₂
+    have h_offset := mem_offsets_of_lt_32 h₂
+    fin_cases h_offset
+    all_goals aesop
+
+abbrev Entry := UInt256 × UInt8
+
+@[simp]
+def memInsert (entry : Entry) (mem : Memory) : Memory :=
+  Function.uncurry mem.insert entry
+
+@[simp]
+def mkEntries (addr data : UInt256) : List Entry :=
+  let addrs := offsets.map (addr + ↑·)
+  addrs.zip (UInt256.toBytes! data)
+
+def Memory.maxWords := 3618502788666131106986593281521497120414687020801267626233049500247285301247
+
+def Memory.maxWords_def : Memory.maxWords = (⊤ : UInt256) / 32 := by
+  rw [maxWords, Fin.top_eq_last]
+  simp
+
 def MachineState.updateMemory (m : MachineState) (addr v : UInt256) : MachineState :=
-  {m with memory := let offsets := List.range 32
-                    let addrs   := offsets.map (·+addr)
-                    let inserts := addrs.zipWith Finmap.insert (UInt256.toBytes! v)
-                    inserts.foldl (init := m.memory) (flip id)
+  {m with memory := List.foldr (init := m.memory) memInsert <| mkEntries addr v
           max_address := max addr m.max_address }
 
-lemma cheeky_proof {a b : Int} : (if a > b then a else b) = max a b := by rw [max_comm, max_def_lt]
+def Memory.lookupByte (m : Memory) (addr : UInt256) : UInt8 :=
+  (m.lookup addr).get!
 
-def MachineState.lookupMemory (m : MachineState) (addr : UInt256) : UInt256 :=
-  UInt256.fromBytes! (List.map (fun i => (m.memory.lookup (addr + i)).get!) UInt256.offsets)
+def Memory.lookupWord (m : Memory) (addr : UInt256) : UInt256 :=
+--  UInt256.fromBytes! (offsets.map λ i ↦ (m.memory.lookup (addr + i)).get!)
+  UInt256.fromBytes! $ offsets.map $ m.lookupByte ∘ (addr + ↑·)
 
 def MachineState.setReturnData (m : MachineState) (r : List UInt256) : MachineState :=
   {m with return_data := r}
 
 def MachineState.msize (m : MachineState) : UInt256 :=
   m.max_address
-
 
 -- definition of the blocks
 
@@ -163,6 +323,11 @@ instance : Inhabited EVMState :=
 
 abbrev EVM := EVMState
 
+def preserved : EVMState → EVMState → Prop :=
+  (Eq on EVMState.account_map) ∩
+  (Eq on EVMState.hash_collision) ∩
+  (Eq on EVMState.execution_env)
+
 -- functions for querying balance
 
 namespace EVMState
@@ -172,7 +337,12 @@ section
 open Array ByteArray
 
 -- | Add an error to the EVMState indicating that we hit a hash collision in `keccak256`.
-def addHashCollision (σ : EVMState) : EVMState := { σ with hash_collision := True }
+def addHashCollision (σ : EVMState) : EVMState := { σ with hash_collision := true }
+
+-- def hasHashCollision (σ : EVMState) : Prop := σ.hash_collision = true
+
+-- instance : DecidablePred hasHashCollision := λ σ ↦
+--   decidable_of_bool σ.hash_collision (by unfold hasHashCollision; simp)
 
 def lookupAccount (σ : EVMState) (addr : Address) : Option Account :=
   σ.account_map.lookup addr
@@ -202,14 +372,20 @@ def calldatacopy (σ : EVMState) (mstart datastart s : UInt256) : EVMState :=
   let r := arr.foldl (λ (sa , j) i => (EVMState.updateMemory sa j i.val, j + 1)) (σ , mstart)
   r.1
 
-def mkInterval (ms : MachineState) (p n : UInt256) : List UInt256 :=
-  let i : ℕ := p.val
-  let f : ℕ := n.val
-  let m     := (List.range' i f).map Fin.ofNat
-  m.map ms.lookupMemory
+def mkInterval (ms : Memory) (p : UInt256) (n : ℕ) : List UInt256 :=
+  (words_at p n).map ms.lookupWord
+
+def mkInterval' (ms : Memory) (start last : UInt256) : List UInt8 :=
+  List.map ms.lookupByte <| range' start (last - start)
+
+lemma interval'_eq_interval {ms} {start last} (d : ℕ) :
+  (d_ne_zero : d ≠ 0) → (div : (d * 32) * Fin.div (last - start) (Nat.toUInt256 d * 32) = last - start) →
+  List.map (Nat.toUInt256 ∘ fromBytes!) (List.toChunks 32 (mkInterval' ms start last)) =
+    mkInterval ms start d := by
+  sorry
 
 def keccak256 (σ : EVMState) (p n : UInt256) : Option (UInt256 × EVMState) :=
-  let interval : List UInt256 := mkInterval σ.machine_state p n
+  let interval : List UInt256 := List.map (Nat.toUInt256 ∘ fromBytes!) (List.toChunks 32 (mkInterval' σ.machine_state.memory p n))
   match Finmap.lookup interval σ.keccak_map with
   | .some val => .some (val, σ)
   | .none     =>
@@ -290,7 +466,7 @@ def selfbalance (σ : EVMState) : UInt256 :=
 -- memory and storage operations
 
 def mload (σ : EVMState) (spos : UInt256) : UInt256 :=
-  σ.machine_state.lookupMemory spos
+  σ.machine_state.memory.lookupWord spos
 
 def mstore (σ : EVMState) (spos sval : UInt256) : EVMState :=
   σ.updateMemory spos sval
@@ -340,5 +516,1329 @@ def evm_revert (σ : EVMState) (mstart s : UInt256) : EVMState :=
   σ.evm_return mstart s
 
 end
+
+section Memory
+
+variable {addr addr' : UInt256}
+variable {ms : MachineState}
+variable {val val' : UInt256}
+variable {entry : Entry}
+variable {es es' : List Entry}
+
+@[simp]
+lemma frontflip : (λ b a ↦ memInsert a b) = flip memInsert := by
+  unfold flip
+  ext
+  simp
+
+@[simp]
+lemma backflip : (λ b a ↦ flip memInsert a b) = memInsert := by
+  unfold flip
+  ext
+  simp
+
+lemma foldr_mem_nil {init : Memory} :
+  List.foldr memInsert (List.foldr memInsert init []) [] = init := by
+  simp
+
+lemma memInsert_memInsert {m : Memory} {a b : UInt8} :
+  memInsert ⟨addr, a⟩ (memInsert ⟨addr, b⟩ m) =
+    memInsert ⟨addr, a⟩ m := by
+  simp
+
+lemma memInsert_memInsert_of_ne {m : Memory} {a b : UInt8} :
+  (h : addr' ≠ addr) →
+  memInsert ⟨addr, a⟩ (memInsert ⟨addr', b⟩ m) =
+    memInsert ⟨addr', b⟩ (memInsert ⟨addr, a⟩ m) := by
+  intro h
+  simp
+  exact Finmap.insert_insert_of_ne m h
+
+lemma foldr_memInsert_reverse {init : Memory} :
+  List.foldr memInsert init (mkEntries addr val) =
+    List.foldr memInsert init (mkEntries addr val).reverse := by
+  simp only [mkEntries]
+  rw [ splice_toBytes! val ]
+  unfold offsets
+
+  simp only [List.map, List.zip, List.zipWith, List.reverse, List.reverseAux]
+  simp only [Nat.cast_ofNat, Nat.cast_one, Nat.cast_zero]
+  rw [List.foldr_cons]
+  rw [ List.foldr_cons
+     , memInsert_memInsert_of_ne (b := (toBytes! val)[1]) (by simp)
+     ]
+  rw [ List.foldr_cons
+     , memInsert_memInsert_of_ne (b := (toBytes! val)[2]) (by simp)
+     , memInsert_memInsert_of_ne (b := (toBytes! val)[2]) (by simp)
+     ]
+  rw [ List.foldr_cons
+     , memInsert_memInsert_of_ne (b := (toBytes! val)[3]) (by simp)
+     , memInsert_memInsert_of_ne (b := (toBytes! val)[3]) (by simp)
+     , memInsert_memInsert_of_ne (b := (toBytes! val)[3]) (by simp)
+     ]
+  rw [ List.foldr_cons
+     , memInsert_memInsert_of_ne (b := (toBytes! val)[4]) (by simp)
+     , memInsert_memInsert_of_ne (b := (toBytes! val)[4]) (by simp)
+     , memInsert_memInsert_of_ne (b := (toBytes! val)[4]) (by simp)
+     , memInsert_memInsert_of_ne (b := (toBytes! val)[4]) (by simp)
+     ]
+  rw [ List.foldr_cons
+     , memInsert_memInsert_of_ne (b := (toBytes! val)[5]) (by simp)
+     , memInsert_memInsert_of_ne (b := (toBytes! val)[5]) (by simp)
+     , memInsert_memInsert_of_ne (b := (toBytes! val)[5]) (by simp)
+     , memInsert_memInsert_of_ne (b := (toBytes! val)[5]) (by simp)
+     , memInsert_memInsert_of_ne (b := (toBytes! val)[5]) (by simp)
+     ]
+  rw [ List.foldr_cons
+     , memInsert_memInsert_of_ne (b := (toBytes! val)[6]) (by simp)
+     , memInsert_memInsert_of_ne (b := (toBytes! val)[6]) (by simp)
+     , memInsert_memInsert_of_ne (b := (toBytes! val)[6]) (by simp)
+     , memInsert_memInsert_of_ne (b := (toBytes! val)[6]) (by simp)
+     , memInsert_memInsert_of_ne (b := (toBytes! val)[6]) (by simp)
+     , memInsert_memInsert_of_ne (b := (toBytes! val)[6]) (by simp)
+     ]
+  rw [ List.foldr_cons
+     , memInsert_memInsert_of_ne (b := (toBytes! val)[7]) (by simp)
+     , memInsert_memInsert_of_ne (b := (toBytes! val)[7]) (by simp)
+     , memInsert_memInsert_of_ne (b := (toBytes! val)[7]) (by simp)
+     , memInsert_memInsert_of_ne (b := (toBytes! val)[7]) (by simp)
+     , memInsert_memInsert_of_ne (b := (toBytes! val)[7]) (by simp)
+     , memInsert_memInsert_of_ne (b := (toBytes! val)[7]) (by simp)
+     , memInsert_memInsert_of_ne (b := (toBytes! val)[7]) (by simp)
+     ]
+  rw [ List.foldr_cons
+     , memInsert_memInsert_of_ne (b := (toBytes! val)[8]) (by simp)
+     , memInsert_memInsert_of_ne (b := (toBytes! val)[8]) (by simp)
+     , memInsert_memInsert_of_ne (b := (toBytes! val)[8]) (by simp)
+     , memInsert_memInsert_of_ne (b := (toBytes! val)[8]) (by simp)
+     , memInsert_memInsert_of_ne (b := (toBytes! val)[8]) (by simp)
+     , memInsert_memInsert_of_ne (b := (toBytes! val)[8]) (by simp)
+     , memInsert_memInsert_of_ne (b := (toBytes! val)[8]) (by simp)
+     , memInsert_memInsert_of_ne (b := (toBytes! val)[8]) (by simp)
+     ]
+  rw [ List.foldr_cons
+     , memInsert_memInsert_of_ne (b := (toBytes! val)[9]) (by simp)
+     , memInsert_memInsert_of_ne (b := (toBytes! val)[9]) (by simp)
+     , memInsert_memInsert_of_ne (b := (toBytes! val)[9]) (by simp)
+     , memInsert_memInsert_of_ne (b := (toBytes! val)[9]) (by simp)
+     , memInsert_memInsert_of_ne (b := (toBytes! val)[9]) (by simp)
+     , memInsert_memInsert_of_ne (b := (toBytes! val)[9]) (by simp)
+     , memInsert_memInsert_of_ne (b := (toBytes! val)[9]) (by simp)
+     , memInsert_memInsert_of_ne (b := (toBytes! val)[9]) (by simp)
+     , memInsert_memInsert_of_ne (b := (toBytes! val)[9]) (by simp)
+     ]
+  rw [ List.foldr_cons
+     , memInsert_memInsert_of_ne (b := (toBytes! val)[10]) (by simp)
+     , memInsert_memInsert_of_ne (b := (toBytes! val)[10]) (by simp)
+     , memInsert_memInsert_of_ne (b := (toBytes! val)[10]) (by simp)
+     , memInsert_memInsert_of_ne (b := (toBytes! val)[10]) (by simp)
+     , memInsert_memInsert_of_ne (b := (toBytes! val)[10]) (by simp)
+     , memInsert_memInsert_of_ne (b := (toBytes! val)[10]) (by simp)
+     , memInsert_memInsert_of_ne (b := (toBytes! val)[10]) (by simp)
+     , memInsert_memInsert_of_ne (b := (toBytes! val)[10]) (by simp)
+     , memInsert_memInsert_of_ne (b := (toBytes! val)[10]) (by simp)
+     , memInsert_memInsert_of_ne (b := (toBytes! val)[10]) (by simp)
+     ]
+  rw [ List.foldr_cons
+     , memInsert_memInsert_of_ne (b := (toBytes! val)[11]) (by simp)
+     , memInsert_memInsert_of_ne (b := (toBytes! val)[11]) (by simp)
+     , memInsert_memInsert_of_ne (b := (toBytes! val)[11]) (by simp)
+     , memInsert_memInsert_of_ne (b := (toBytes! val)[11]) (by simp)
+     , memInsert_memInsert_of_ne (b := (toBytes! val)[11]) (by simp)
+     , memInsert_memInsert_of_ne (b := (toBytes! val)[11]) (by simp)
+     , memInsert_memInsert_of_ne (b := (toBytes! val)[11]) (by simp)
+     , memInsert_memInsert_of_ne (b := (toBytes! val)[11]) (by simp)
+     , memInsert_memInsert_of_ne (b := (toBytes! val)[11]) (by simp)
+     , memInsert_memInsert_of_ne (b := (toBytes! val)[11]) (by simp)
+     , memInsert_memInsert_of_ne (b := (toBytes! val)[11]) (by simp)
+     ]
+  rw [ List.foldr_cons
+     , memInsert_memInsert_of_ne (b := (toBytes! val)[12]) (by simp)
+     , memInsert_memInsert_of_ne (b := (toBytes! val)[12]) (by simp)
+     , memInsert_memInsert_of_ne (b := (toBytes! val)[12]) (by simp)
+     , memInsert_memInsert_of_ne (b := (toBytes! val)[12]) (by simp)
+     , memInsert_memInsert_of_ne (b := (toBytes! val)[12]) (by simp)
+     , memInsert_memInsert_of_ne (b := (toBytes! val)[12]) (by simp)
+     , memInsert_memInsert_of_ne (b := (toBytes! val)[12]) (by simp)
+     , memInsert_memInsert_of_ne (b := (toBytes! val)[12]) (by simp)
+     , memInsert_memInsert_of_ne (b := (toBytes! val)[12]) (by simp)
+     , memInsert_memInsert_of_ne (b := (toBytes! val)[12]) (by simp)
+     , memInsert_memInsert_of_ne (b := (toBytes! val)[12]) (by simp)
+     , memInsert_memInsert_of_ne (b := (toBytes! val)[12]) (by simp)
+     ]
+  rw [ List.foldr_cons
+     , memInsert_memInsert_of_ne (b := (toBytes! val)[13]) (by simp)
+     , memInsert_memInsert_of_ne (b := (toBytes! val)[13]) (by simp)
+     , memInsert_memInsert_of_ne (b := (toBytes! val)[13]) (by simp)
+     , memInsert_memInsert_of_ne (b := (toBytes! val)[13]) (by simp)
+     , memInsert_memInsert_of_ne (b := (toBytes! val)[13]) (by simp)
+     , memInsert_memInsert_of_ne (b := (toBytes! val)[13]) (by simp)
+     , memInsert_memInsert_of_ne (b := (toBytes! val)[13]) (by simp)
+     , memInsert_memInsert_of_ne (b := (toBytes! val)[13]) (by simp)
+     , memInsert_memInsert_of_ne (b := (toBytes! val)[13]) (by simp)
+     , memInsert_memInsert_of_ne (b := (toBytes! val)[13]) (by simp)
+     , memInsert_memInsert_of_ne (b := (toBytes! val)[13]) (by simp)
+     , memInsert_memInsert_of_ne (b := (toBytes! val)[13]) (by simp)
+     , memInsert_memInsert_of_ne (b := (toBytes! val)[13]) (by simp)
+     ]
+  rw [ List.foldr_cons
+     , memInsert_memInsert_of_ne (b := (toBytes! val)[14]) (by simp)
+     , memInsert_memInsert_of_ne (b := (toBytes! val)[14]) (by simp)
+     , memInsert_memInsert_of_ne (b := (toBytes! val)[14]) (by simp)
+     , memInsert_memInsert_of_ne (b := (toBytes! val)[14]) (by simp)
+     , memInsert_memInsert_of_ne (b := (toBytes! val)[14]) (by simp)
+     , memInsert_memInsert_of_ne (b := (toBytes! val)[14]) (by simp)
+     , memInsert_memInsert_of_ne (b := (toBytes! val)[14]) (by simp)
+     , memInsert_memInsert_of_ne (b := (toBytes! val)[14]) (by simp)
+     , memInsert_memInsert_of_ne (b := (toBytes! val)[14]) (by simp)
+     , memInsert_memInsert_of_ne (b := (toBytes! val)[14]) (by simp)
+     , memInsert_memInsert_of_ne (b := (toBytes! val)[14]) (by simp)
+     , memInsert_memInsert_of_ne (b := (toBytes! val)[14]) (by simp)
+     , memInsert_memInsert_of_ne (b := (toBytes! val)[14]) (by simp)
+     , memInsert_memInsert_of_ne (b := (toBytes! val)[14]) (by simp)
+     ]
+  rw [ List.foldr_cons
+     , memInsert_memInsert_of_ne (b := (toBytes! val)[15]) (by simp)
+     , memInsert_memInsert_of_ne (b := (toBytes! val)[15]) (by simp)
+     , memInsert_memInsert_of_ne (b := (toBytes! val)[15]) (by simp)
+     , memInsert_memInsert_of_ne (b := (toBytes! val)[15]) (by simp)
+     , memInsert_memInsert_of_ne (b := (toBytes! val)[15]) (by simp)
+     , memInsert_memInsert_of_ne (b := (toBytes! val)[15]) (by simp)
+     , memInsert_memInsert_of_ne (b := (toBytes! val)[15]) (by simp)
+     , memInsert_memInsert_of_ne (b := (toBytes! val)[15]) (by simp)
+     , memInsert_memInsert_of_ne (b := (toBytes! val)[15]) (by simp)
+     , memInsert_memInsert_of_ne (b := (toBytes! val)[15]) (by simp)
+     , memInsert_memInsert_of_ne (b := (toBytes! val)[15]) (by simp)
+     , memInsert_memInsert_of_ne (b := (toBytes! val)[15]) (by simp)
+     , memInsert_memInsert_of_ne (b := (toBytes! val)[15]) (by simp)
+     , memInsert_memInsert_of_ne (b := (toBytes! val)[15]) (by simp)
+     , memInsert_memInsert_of_ne (b := (toBytes! val)[15]) (by simp)
+     ]
+  rw [ List.foldr_cons
+     , memInsert_memInsert_of_ne (b := (toBytes! val)[16]) (by simp)
+     , memInsert_memInsert_of_ne (b := (toBytes! val)[16]) (by simp)
+     , memInsert_memInsert_of_ne (b := (toBytes! val)[16]) (by simp)
+     , memInsert_memInsert_of_ne (b := (toBytes! val)[16]) (by simp)
+     , memInsert_memInsert_of_ne (b := (toBytes! val)[16]) (by simp)
+     , memInsert_memInsert_of_ne (b := (toBytes! val)[16]) (by simp)
+     , memInsert_memInsert_of_ne (b := (toBytes! val)[16]) (by simp)
+     , memInsert_memInsert_of_ne (b := (toBytes! val)[16]) (by simp)
+     , memInsert_memInsert_of_ne (b := (toBytes! val)[16]) (by simp)
+     , memInsert_memInsert_of_ne (b := (toBytes! val)[16]) (by simp)
+     , memInsert_memInsert_of_ne (b := (toBytes! val)[16]) (by simp)
+     , memInsert_memInsert_of_ne (b := (toBytes! val)[16]) (by simp)
+     , memInsert_memInsert_of_ne (b := (toBytes! val)[16]) (by simp)
+     , memInsert_memInsert_of_ne (b := (toBytes! val)[16]) (by simp)
+     , memInsert_memInsert_of_ne (b := (toBytes! val)[16]) (by simp)
+     , memInsert_memInsert_of_ne (b := (toBytes! val)[16]) (by simp)
+     ]
+  rw [ List.foldr_cons
+     , memInsert_memInsert_of_ne (b := (toBytes! val)[17]) (by simp)
+     , memInsert_memInsert_of_ne (b := (toBytes! val)[17]) (by simp)
+     , memInsert_memInsert_of_ne (b := (toBytes! val)[17]) (by simp)
+     , memInsert_memInsert_of_ne (b := (toBytes! val)[17]) (by simp)
+     , memInsert_memInsert_of_ne (b := (toBytes! val)[17]) (by simp)
+     , memInsert_memInsert_of_ne (b := (toBytes! val)[17]) (by simp)
+     , memInsert_memInsert_of_ne (b := (toBytes! val)[17]) (by simp)
+     , memInsert_memInsert_of_ne (b := (toBytes! val)[17]) (by simp)
+     , memInsert_memInsert_of_ne (b := (toBytes! val)[17]) (by simp)
+     , memInsert_memInsert_of_ne (b := (toBytes! val)[17]) (by simp)
+     , memInsert_memInsert_of_ne (b := (toBytes! val)[17]) (by simp)
+     , memInsert_memInsert_of_ne (b := (toBytes! val)[17]) (by simp)
+     , memInsert_memInsert_of_ne (b := (toBytes! val)[17]) (by simp)
+     , memInsert_memInsert_of_ne (b := (toBytes! val)[17]) (by simp)
+     , memInsert_memInsert_of_ne (b := (toBytes! val)[17]) (by simp)
+     , memInsert_memInsert_of_ne (b := (toBytes! val)[17]) (by simp)
+     , memInsert_memInsert_of_ne (b := (toBytes! val)[17]) (by simp)
+     ]
+  rw [ List.foldr_cons
+     , memInsert_memInsert_of_ne (b := (toBytes! val)[18]) (by simp)
+     , memInsert_memInsert_of_ne (b := (toBytes! val)[18]) (by simp)
+     , memInsert_memInsert_of_ne (b := (toBytes! val)[18]) (by simp)
+     , memInsert_memInsert_of_ne (b := (toBytes! val)[18]) (by simp)
+     , memInsert_memInsert_of_ne (b := (toBytes! val)[18]) (by simp)
+     , memInsert_memInsert_of_ne (b := (toBytes! val)[18]) (by simp)
+     , memInsert_memInsert_of_ne (b := (toBytes! val)[18]) (by simp)
+     , memInsert_memInsert_of_ne (b := (toBytes! val)[18]) (by simp)
+     , memInsert_memInsert_of_ne (b := (toBytes! val)[18]) (by simp)
+     , memInsert_memInsert_of_ne (b := (toBytes! val)[18]) (by simp)
+     , memInsert_memInsert_of_ne (b := (toBytes! val)[18]) (by simp)
+     , memInsert_memInsert_of_ne (b := (toBytes! val)[18]) (by simp)
+     , memInsert_memInsert_of_ne (b := (toBytes! val)[18]) (by simp)
+     , memInsert_memInsert_of_ne (b := (toBytes! val)[18]) (by simp)
+     , memInsert_memInsert_of_ne (b := (toBytes! val)[18]) (by simp)
+     , memInsert_memInsert_of_ne (b := (toBytes! val)[18]) (by simp)
+     , memInsert_memInsert_of_ne (b := (toBytes! val)[18]) (by simp)
+     , memInsert_memInsert_of_ne (b := (toBytes! val)[18]) (by simp)
+     ]
+  rw [ List.foldr_cons
+     , memInsert_memInsert_of_ne (b := (toBytes! val)[19]) (by simp)
+     , memInsert_memInsert_of_ne (b := (toBytes! val)[19]) (by simp)
+     , memInsert_memInsert_of_ne (b := (toBytes! val)[19]) (by simp)
+     , memInsert_memInsert_of_ne (b := (toBytes! val)[19]) (by simp)
+     , memInsert_memInsert_of_ne (b := (toBytes! val)[19]) (by simp)
+     , memInsert_memInsert_of_ne (b := (toBytes! val)[19]) (by simp)
+     , memInsert_memInsert_of_ne (b := (toBytes! val)[19]) (by simp)
+     , memInsert_memInsert_of_ne (b := (toBytes! val)[19]) (by simp)
+     , memInsert_memInsert_of_ne (b := (toBytes! val)[19]) (by simp)
+     , memInsert_memInsert_of_ne (b := (toBytes! val)[19]) (by simp)
+     , memInsert_memInsert_of_ne (b := (toBytes! val)[19]) (by simp)
+     , memInsert_memInsert_of_ne (b := (toBytes! val)[19]) (by simp)
+     , memInsert_memInsert_of_ne (b := (toBytes! val)[19]) (by simp)
+     , memInsert_memInsert_of_ne (b := (toBytes! val)[19]) (by simp)
+     , memInsert_memInsert_of_ne (b := (toBytes! val)[19]) (by simp)
+     , memInsert_memInsert_of_ne (b := (toBytes! val)[19]) (by simp)
+     , memInsert_memInsert_of_ne (b := (toBytes! val)[19]) (by simp)
+     , memInsert_memInsert_of_ne (b := (toBytes! val)[19]) (by simp)
+     , memInsert_memInsert_of_ne (b := (toBytes! val)[19]) (by simp)
+     ]
+  rw [ List.foldr_cons
+     , memInsert_memInsert_of_ne (b := (toBytes! val)[20]) (by simp)
+     , memInsert_memInsert_of_ne (b := (toBytes! val)[20]) (by simp)
+     , memInsert_memInsert_of_ne (b := (toBytes! val)[20]) (by simp)
+     , memInsert_memInsert_of_ne (b := (toBytes! val)[20]) (by simp)
+     , memInsert_memInsert_of_ne (b := (toBytes! val)[20]) (by simp)
+     , memInsert_memInsert_of_ne (b := (toBytes! val)[20]) (by simp)
+     , memInsert_memInsert_of_ne (b := (toBytes! val)[20]) (by simp)
+     , memInsert_memInsert_of_ne (b := (toBytes! val)[20]) (by simp)
+     , memInsert_memInsert_of_ne (b := (toBytes! val)[20]) (by simp)
+     , memInsert_memInsert_of_ne (b := (toBytes! val)[20]) (by simp)
+     , memInsert_memInsert_of_ne (b := (toBytes! val)[20]) (by simp)
+     , memInsert_memInsert_of_ne (b := (toBytes! val)[20]) (by simp)
+     , memInsert_memInsert_of_ne (b := (toBytes! val)[20]) (by simp)
+     , memInsert_memInsert_of_ne (b := (toBytes! val)[20]) (by simp)
+     , memInsert_memInsert_of_ne (b := (toBytes! val)[20]) (by simp)
+     , memInsert_memInsert_of_ne (b := (toBytes! val)[20]) (by simp)
+     , memInsert_memInsert_of_ne (b := (toBytes! val)[20]) (by simp)
+     , memInsert_memInsert_of_ne (b := (toBytes! val)[20]) (by simp)
+     , memInsert_memInsert_of_ne (b := (toBytes! val)[20]) (by simp)
+     , memInsert_memInsert_of_ne (b := (toBytes! val)[20]) (by simp)
+     ]
+  rw [ List.foldr_cons
+     , memInsert_memInsert_of_ne (b := (toBytes! val)[21]) (by simp)
+     , memInsert_memInsert_of_ne (b := (toBytes! val)[21]) (by simp)
+     , memInsert_memInsert_of_ne (b := (toBytes! val)[21]) (by simp)
+     , memInsert_memInsert_of_ne (b := (toBytes! val)[21]) (by simp)
+     , memInsert_memInsert_of_ne (b := (toBytes! val)[21]) (by simp)
+     , memInsert_memInsert_of_ne (b := (toBytes! val)[21]) (by simp)
+     , memInsert_memInsert_of_ne (b := (toBytes! val)[21]) (by simp)
+     , memInsert_memInsert_of_ne (b := (toBytes! val)[21]) (by simp)
+     , memInsert_memInsert_of_ne (b := (toBytes! val)[21]) (by simp)
+     , memInsert_memInsert_of_ne (b := (toBytes! val)[21]) (by simp)
+     , memInsert_memInsert_of_ne (b := (toBytes! val)[21]) (by simp)
+     , memInsert_memInsert_of_ne (b := (toBytes! val)[21]) (by simp)
+     , memInsert_memInsert_of_ne (b := (toBytes! val)[21]) (by simp)
+     , memInsert_memInsert_of_ne (b := (toBytes! val)[21]) (by simp)
+     , memInsert_memInsert_of_ne (b := (toBytes! val)[21]) (by simp)
+     , memInsert_memInsert_of_ne (b := (toBytes! val)[21]) (by simp)
+     , memInsert_memInsert_of_ne (b := (toBytes! val)[21]) (by simp)
+     , memInsert_memInsert_of_ne (b := (toBytes! val)[21]) (by simp)
+     , memInsert_memInsert_of_ne (b := (toBytes! val)[21]) (by simp)
+     , memInsert_memInsert_of_ne (b := (toBytes! val)[21]) (by simp)
+     , memInsert_memInsert_of_ne (b := (toBytes! val)[21]) (by simp)
+     ]
+  rw [ List.foldr_cons
+     , memInsert_memInsert_of_ne (b := (toBytes! val)[22]) (by simp)
+     , memInsert_memInsert_of_ne (b := (toBytes! val)[22]) (by simp)
+     , memInsert_memInsert_of_ne (b := (toBytes! val)[22]) (by simp)
+     , memInsert_memInsert_of_ne (b := (toBytes! val)[22]) (by simp)
+     , memInsert_memInsert_of_ne (b := (toBytes! val)[22]) (by simp)
+     , memInsert_memInsert_of_ne (b := (toBytes! val)[22]) (by simp)
+     , memInsert_memInsert_of_ne (b := (toBytes! val)[22]) (by simp)
+     , memInsert_memInsert_of_ne (b := (toBytes! val)[22]) (by simp)
+     , memInsert_memInsert_of_ne (b := (toBytes! val)[22]) (by simp)
+     , memInsert_memInsert_of_ne (b := (toBytes! val)[22]) (by simp)
+     , memInsert_memInsert_of_ne (b := (toBytes! val)[22]) (by simp)
+     , memInsert_memInsert_of_ne (b := (toBytes! val)[22]) (by simp)
+     , memInsert_memInsert_of_ne (b := (toBytes! val)[22]) (by simp)
+     , memInsert_memInsert_of_ne (b := (toBytes! val)[22]) (by simp)
+     , memInsert_memInsert_of_ne (b := (toBytes! val)[22]) (by simp)
+     , memInsert_memInsert_of_ne (b := (toBytes! val)[22]) (by simp)
+     , memInsert_memInsert_of_ne (b := (toBytes! val)[22]) (by simp)
+     , memInsert_memInsert_of_ne (b := (toBytes! val)[22]) (by simp)
+     , memInsert_memInsert_of_ne (b := (toBytes! val)[22]) (by simp)
+     , memInsert_memInsert_of_ne (b := (toBytes! val)[22]) (by simp)
+     , memInsert_memInsert_of_ne (b := (toBytes! val)[22]) (by simp)
+     , memInsert_memInsert_of_ne (b := (toBytes! val)[22]) (by simp)
+     ]
+  rw [ List.foldr_cons
+     , memInsert_memInsert_of_ne (b := (toBytes! val)[23]) (by simp)
+     , memInsert_memInsert_of_ne (b := (toBytes! val)[23]) (by simp)
+     , memInsert_memInsert_of_ne (b := (toBytes! val)[23]) (by simp)
+     , memInsert_memInsert_of_ne (b := (toBytes! val)[23]) (by simp)
+     , memInsert_memInsert_of_ne (b := (toBytes! val)[23]) (by simp)
+     , memInsert_memInsert_of_ne (b := (toBytes! val)[23]) (by simp)
+     , memInsert_memInsert_of_ne (b := (toBytes! val)[23]) (by simp)
+     , memInsert_memInsert_of_ne (b := (toBytes! val)[23]) (by simp)
+     , memInsert_memInsert_of_ne (b := (toBytes! val)[23]) (by simp)
+     , memInsert_memInsert_of_ne (b := (toBytes! val)[23]) (by simp)
+     , memInsert_memInsert_of_ne (b := (toBytes! val)[23]) (by simp)
+     , memInsert_memInsert_of_ne (b := (toBytes! val)[23]) (by simp)
+     , memInsert_memInsert_of_ne (b := (toBytes! val)[23]) (by simp)
+     , memInsert_memInsert_of_ne (b := (toBytes! val)[23]) (by simp)
+     , memInsert_memInsert_of_ne (b := (toBytes! val)[23]) (by simp)
+     , memInsert_memInsert_of_ne (b := (toBytes! val)[23]) (by simp)
+     , memInsert_memInsert_of_ne (b := (toBytes! val)[23]) (by simp)
+     , memInsert_memInsert_of_ne (b := (toBytes! val)[23]) (by simp)
+     , memInsert_memInsert_of_ne (b := (toBytes! val)[23]) (by simp)
+     , memInsert_memInsert_of_ne (b := (toBytes! val)[23]) (by simp)
+     , memInsert_memInsert_of_ne (b := (toBytes! val)[23]) (by simp)
+     , memInsert_memInsert_of_ne (b := (toBytes! val)[23]) (by simp)
+     , memInsert_memInsert_of_ne (b := (toBytes! val)[23]) (by simp)
+     ]
+  rw [ List.foldr_cons
+     , memInsert_memInsert_of_ne (b := (toBytes! val)[24]) (by simp)
+     , memInsert_memInsert_of_ne (b := (toBytes! val)[24]) (by simp)
+     , memInsert_memInsert_of_ne (b := (toBytes! val)[24]) (by simp)
+     , memInsert_memInsert_of_ne (b := (toBytes! val)[24]) (by simp)
+     , memInsert_memInsert_of_ne (b := (toBytes! val)[24]) (by simp)
+     , memInsert_memInsert_of_ne (b := (toBytes! val)[24]) (by simp)
+     , memInsert_memInsert_of_ne (b := (toBytes! val)[24]) (by simp)
+     , memInsert_memInsert_of_ne (b := (toBytes! val)[24]) (by simp)
+     , memInsert_memInsert_of_ne (b := (toBytes! val)[24]) (by simp)
+     , memInsert_memInsert_of_ne (b := (toBytes! val)[24]) (by simp)
+     , memInsert_memInsert_of_ne (b := (toBytes! val)[24]) (by simp)
+     , memInsert_memInsert_of_ne (b := (toBytes! val)[24]) (by simp)
+     , memInsert_memInsert_of_ne (b := (toBytes! val)[24]) (by simp)
+     , memInsert_memInsert_of_ne (b := (toBytes! val)[24]) (by simp)
+     , memInsert_memInsert_of_ne (b := (toBytes! val)[24]) (by simp)
+     , memInsert_memInsert_of_ne (b := (toBytes! val)[24]) (by simp)
+     , memInsert_memInsert_of_ne (b := (toBytes! val)[24]) (by simp)
+     , memInsert_memInsert_of_ne (b := (toBytes! val)[24]) (by simp)
+     , memInsert_memInsert_of_ne (b := (toBytes! val)[24]) (by simp)
+     , memInsert_memInsert_of_ne (b := (toBytes! val)[24]) (by simp)
+     , memInsert_memInsert_of_ne (b := (toBytes! val)[24]) (by simp)
+     , memInsert_memInsert_of_ne (b := (toBytes! val)[24]) (by simp)
+     , memInsert_memInsert_of_ne (b := (toBytes! val)[24]) (by simp)
+     , memInsert_memInsert_of_ne (b := (toBytes! val)[24]) (by simp)
+     ]
+  rw [ List.foldr_cons
+     , memInsert_memInsert_of_ne (b := (toBytes! val)[25]) (by simp)
+     , memInsert_memInsert_of_ne (b := (toBytes! val)[25]) (by simp)
+     , memInsert_memInsert_of_ne (b := (toBytes! val)[25]) (by simp)
+     , memInsert_memInsert_of_ne (b := (toBytes! val)[25]) (by simp)
+     , memInsert_memInsert_of_ne (b := (toBytes! val)[25]) (by simp)
+     , memInsert_memInsert_of_ne (b := (toBytes! val)[25]) (by simp)
+     , memInsert_memInsert_of_ne (b := (toBytes! val)[25]) (by simp)
+     , memInsert_memInsert_of_ne (b := (toBytes! val)[25]) (by simp)
+     , memInsert_memInsert_of_ne (b := (toBytes! val)[25]) (by simp)
+     , memInsert_memInsert_of_ne (b := (toBytes! val)[25]) (by simp)
+     , memInsert_memInsert_of_ne (b := (toBytes! val)[25]) (by simp)
+     , memInsert_memInsert_of_ne (b := (toBytes! val)[25]) (by simp)
+     , memInsert_memInsert_of_ne (b := (toBytes! val)[25]) (by simp)
+     , memInsert_memInsert_of_ne (b := (toBytes! val)[25]) (by simp)
+     , memInsert_memInsert_of_ne (b := (toBytes! val)[25]) (by simp)
+     , memInsert_memInsert_of_ne (b := (toBytes! val)[25]) (by simp)
+     , memInsert_memInsert_of_ne (b := (toBytes! val)[25]) (by simp)
+     , memInsert_memInsert_of_ne (b := (toBytes! val)[25]) (by simp)
+     , memInsert_memInsert_of_ne (b := (toBytes! val)[25]) (by simp)
+     , memInsert_memInsert_of_ne (b := (toBytes! val)[25]) (by simp)
+     , memInsert_memInsert_of_ne (b := (toBytes! val)[25]) (by simp)
+     , memInsert_memInsert_of_ne (b := (toBytes! val)[25]) (by simp)
+     , memInsert_memInsert_of_ne (b := (toBytes! val)[25]) (by simp)
+     , memInsert_memInsert_of_ne (b := (toBytes! val)[25]) (by simp)
+     , memInsert_memInsert_of_ne (b := (toBytes! val)[25]) (by simp)
+     ]
+  rw [ List.foldr_cons
+     , memInsert_memInsert_of_ne (b := (toBytes! val)[26]) (by simp)
+     , memInsert_memInsert_of_ne (b := (toBytes! val)[26]) (by simp)
+     , memInsert_memInsert_of_ne (b := (toBytes! val)[26]) (by simp)
+     , memInsert_memInsert_of_ne (b := (toBytes! val)[26]) (by simp)
+     , memInsert_memInsert_of_ne (b := (toBytes! val)[26]) (by simp)
+     , memInsert_memInsert_of_ne (b := (toBytes! val)[26]) (by simp)
+     , memInsert_memInsert_of_ne (b := (toBytes! val)[26]) (by simp)
+     , memInsert_memInsert_of_ne (b := (toBytes! val)[26]) (by simp)
+     , memInsert_memInsert_of_ne (b := (toBytes! val)[26]) (by simp)
+     , memInsert_memInsert_of_ne (b := (toBytes! val)[26]) (by simp)
+     , memInsert_memInsert_of_ne (b := (toBytes! val)[26]) (by simp)
+     , memInsert_memInsert_of_ne (b := (toBytes! val)[26]) (by simp)
+     , memInsert_memInsert_of_ne (b := (toBytes! val)[26]) (by simp)
+     , memInsert_memInsert_of_ne (b := (toBytes! val)[26]) (by simp)
+     , memInsert_memInsert_of_ne (b := (toBytes! val)[26]) (by simp)
+     , memInsert_memInsert_of_ne (b := (toBytes! val)[26]) (by simp)
+     , memInsert_memInsert_of_ne (b := (toBytes! val)[26]) (by simp)
+     , memInsert_memInsert_of_ne (b := (toBytes! val)[26]) (by simp)
+     , memInsert_memInsert_of_ne (b := (toBytes! val)[26]) (by simp)
+     , memInsert_memInsert_of_ne (b := (toBytes! val)[26]) (by simp)
+     , memInsert_memInsert_of_ne (b := (toBytes! val)[26]) (by simp)
+     , memInsert_memInsert_of_ne (b := (toBytes! val)[26]) (by simp)
+     , memInsert_memInsert_of_ne (b := (toBytes! val)[26]) (by simp)
+     , memInsert_memInsert_of_ne (b := (toBytes! val)[26]) (by simp)
+     , memInsert_memInsert_of_ne (b := (toBytes! val)[26]) (by simp)
+     , memInsert_memInsert_of_ne (b := (toBytes! val)[26]) (by simp)
+     ]
+  rw [ List.foldr_cons
+     , memInsert_memInsert_of_ne (b := (toBytes! val)[27]) (by simp)
+     , memInsert_memInsert_of_ne (b := (toBytes! val)[27]) (by simp)
+     , memInsert_memInsert_of_ne (b := (toBytes! val)[27]) (by simp)
+     , memInsert_memInsert_of_ne (b := (toBytes! val)[27]) (by simp)
+     , memInsert_memInsert_of_ne (b := (toBytes! val)[27]) (by simp)
+     , memInsert_memInsert_of_ne (b := (toBytes! val)[27]) (by simp)
+     , memInsert_memInsert_of_ne (b := (toBytes! val)[27]) (by simp)
+     , memInsert_memInsert_of_ne (b := (toBytes! val)[27]) (by simp)
+     , memInsert_memInsert_of_ne (b := (toBytes! val)[27]) (by simp)
+     , memInsert_memInsert_of_ne (b := (toBytes! val)[27]) (by simp)
+     , memInsert_memInsert_of_ne (b := (toBytes! val)[27]) (by simp)
+     , memInsert_memInsert_of_ne (b := (toBytes! val)[27]) (by simp)
+     , memInsert_memInsert_of_ne (b := (toBytes! val)[27]) (by simp)
+     , memInsert_memInsert_of_ne (b := (toBytes! val)[27]) (by simp)
+     , memInsert_memInsert_of_ne (b := (toBytes! val)[27]) (by simp)
+     , memInsert_memInsert_of_ne (b := (toBytes! val)[27]) (by simp)
+     , memInsert_memInsert_of_ne (b := (toBytes! val)[27]) (by simp)
+     , memInsert_memInsert_of_ne (b := (toBytes! val)[27]) (by simp)
+     , memInsert_memInsert_of_ne (b := (toBytes! val)[27]) (by simp)
+     , memInsert_memInsert_of_ne (b := (toBytes! val)[27]) (by simp)
+     , memInsert_memInsert_of_ne (b := (toBytes! val)[27]) (by simp)
+     , memInsert_memInsert_of_ne (b := (toBytes! val)[27]) (by simp)
+     , memInsert_memInsert_of_ne (b := (toBytes! val)[27]) (by simp)
+     , memInsert_memInsert_of_ne (b := (toBytes! val)[27]) (by simp)
+     , memInsert_memInsert_of_ne (b := (toBytes! val)[27]) (by simp)
+     , memInsert_memInsert_of_ne (b := (toBytes! val)[27]) (by simp)
+     , memInsert_memInsert_of_ne (b := (toBytes! val)[27]) (by simp)
+     ]
+  rw [ List.foldr_cons
+     , memInsert_memInsert_of_ne (b := (toBytes! val)[28]) (by simp)
+     , memInsert_memInsert_of_ne (b := (toBytes! val)[28]) (by simp)
+     , memInsert_memInsert_of_ne (b := (toBytes! val)[28]) (by simp)
+     , memInsert_memInsert_of_ne (b := (toBytes! val)[28]) (by simp)
+     , memInsert_memInsert_of_ne (b := (toBytes! val)[28]) (by simp)
+     , memInsert_memInsert_of_ne (b := (toBytes! val)[28]) (by simp)
+     , memInsert_memInsert_of_ne (b := (toBytes! val)[28]) (by simp)
+     , memInsert_memInsert_of_ne (b := (toBytes! val)[28]) (by simp)
+     , memInsert_memInsert_of_ne (b := (toBytes! val)[28]) (by simp)
+     , memInsert_memInsert_of_ne (b := (toBytes! val)[28]) (by simp)
+     , memInsert_memInsert_of_ne (b := (toBytes! val)[28]) (by simp)
+     , memInsert_memInsert_of_ne (b := (toBytes! val)[28]) (by simp)
+     , memInsert_memInsert_of_ne (b := (toBytes! val)[28]) (by simp)
+     , memInsert_memInsert_of_ne (b := (toBytes! val)[28]) (by simp)
+     , memInsert_memInsert_of_ne (b := (toBytes! val)[28]) (by simp)
+     , memInsert_memInsert_of_ne (b := (toBytes! val)[28]) (by simp)
+     , memInsert_memInsert_of_ne (b := (toBytes! val)[28]) (by simp)
+     , memInsert_memInsert_of_ne (b := (toBytes! val)[28]) (by simp)
+     , memInsert_memInsert_of_ne (b := (toBytes! val)[28]) (by simp)
+     , memInsert_memInsert_of_ne (b := (toBytes! val)[28]) (by simp)
+     , memInsert_memInsert_of_ne (b := (toBytes! val)[28]) (by simp)
+     , memInsert_memInsert_of_ne (b := (toBytes! val)[28]) (by simp)
+     , memInsert_memInsert_of_ne (b := (toBytes! val)[28]) (by simp)
+     , memInsert_memInsert_of_ne (b := (toBytes! val)[28]) (by simp)
+     , memInsert_memInsert_of_ne (b := (toBytes! val)[28]) (by simp)
+     , memInsert_memInsert_of_ne (b := (toBytes! val)[28]) (by simp)
+     , memInsert_memInsert_of_ne (b := (toBytes! val)[28]) (by simp)
+     , memInsert_memInsert_of_ne (b := (toBytes! val)[28]) (by simp)
+     ]
+  rw [ List.foldr_cons
+     , memInsert_memInsert_of_ne (b := (toBytes! val)[29]) (by simp)
+     , memInsert_memInsert_of_ne (b := (toBytes! val)[29]) (by simp)
+     , memInsert_memInsert_of_ne (b := (toBytes! val)[29]) (by simp)
+     , memInsert_memInsert_of_ne (b := (toBytes! val)[29]) (by simp)
+     , memInsert_memInsert_of_ne (b := (toBytes! val)[29]) (by simp)
+     , memInsert_memInsert_of_ne (b := (toBytes! val)[29]) (by simp)
+     , memInsert_memInsert_of_ne (b := (toBytes! val)[29]) (by simp)
+     , memInsert_memInsert_of_ne (b := (toBytes! val)[29]) (by simp)
+     , memInsert_memInsert_of_ne (b := (toBytes! val)[29]) (by simp)
+     , memInsert_memInsert_of_ne (b := (toBytes! val)[29]) (by simp)
+     , memInsert_memInsert_of_ne (b := (toBytes! val)[29]) (by simp)
+     , memInsert_memInsert_of_ne (b := (toBytes! val)[29]) (by simp)
+     , memInsert_memInsert_of_ne (b := (toBytes! val)[29]) (by simp)
+     , memInsert_memInsert_of_ne (b := (toBytes! val)[29]) (by simp)
+     , memInsert_memInsert_of_ne (b := (toBytes! val)[29]) (by simp)
+     , memInsert_memInsert_of_ne (b := (toBytes! val)[29]) (by simp)
+     , memInsert_memInsert_of_ne (b := (toBytes! val)[29]) (by simp)
+     , memInsert_memInsert_of_ne (b := (toBytes! val)[29]) (by simp)
+     , memInsert_memInsert_of_ne (b := (toBytes! val)[29]) (by simp)
+     , memInsert_memInsert_of_ne (b := (toBytes! val)[29]) (by simp)
+     , memInsert_memInsert_of_ne (b := (toBytes! val)[29]) (by simp)
+     , memInsert_memInsert_of_ne (b := (toBytes! val)[29]) (by simp)
+     , memInsert_memInsert_of_ne (b := (toBytes! val)[29]) (by simp)
+     , memInsert_memInsert_of_ne (b := (toBytes! val)[29]) (by simp)
+     , memInsert_memInsert_of_ne (b := (toBytes! val)[29]) (by simp)
+     , memInsert_memInsert_of_ne (b := (toBytes! val)[29]) (by simp)
+     , memInsert_memInsert_of_ne (b := (toBytes! val)[29]) (by simp)
+     , memInsert_memInsert_of_ne (b := (toBytes! val)[29]) (by simp)
+     , memInsert_memInsert_of_ne (b := (toBytes! val)[29]) (by simp)
+     ]
+  rw [ List.foldr_cons
+     , memInsert_memInsert_of_ne (b := (toBytes! val)[30]) (by simp)
+     , memInsert_memInsert_of_ne (b := (toBytes! val)[30]) (by simp)
+     , memInsert_memInsert_of_ne (b := (toBytes! val)[30]) (by simp)
+     , memInsert_memInsert_of_ne (b := (toBytes! val)[30]) (by simp)
+     , memInsert_memInsert_of_ne (b := (toBytes! val)[30]) (by simp)
+     , memInsert_memInsert_of_ne (b := (toBytes! val)[30]) (by simp)
+     , memInsert_memInsert_of_ne (b := (toBytes! val)[30]) (by simp)
+     , memInsert_memInsert_of_ne (b := (toBytes! val)[30]) (by simp)
+     , memInsert_memInsert_of_ne (b := (toBytes! val)[30]) (by simp)
+     , memInsert_memInsert_of_ne (b := (toBytes! val)[30]) (by simp)
+     , memInsert_memInsert_of_ne (b := (toBytes! val)[30]) (by simp)
+     , memInsert_memInsert_of_ne (b := (toBytes! val)[30]) (by simp)
+     , memInsert_memInsert_of_ne (b := (toBytes! val)[30]) (by simp)
+     , memInsert_memInsert_of_ne (b := (toBytes! val)[30]) (by simp)
+     , memInsert_memInsert_of_ne (b := (toBytes! val)[30]) (by simp)
+     , memInsert_memInsert_of_ne (b := (toBytes! val)[30]) (by simp)
+     , memInsert_memInsert_of_ne (b := (toBytes! val)[30]) (by simp)
+     , memInsert_memInsert_of_ne (b := (toBytes! val)[30]) (by simp)
+     , memInsert_memInsert_of_ne (b := (toBytes! val)[30]) (by simp)
+     , memInsert_memInsert_of_ne (b := (toBytes! val)[30]) (by simp)
+     , memInsert_memInsert_of_ne (b := (toBytes! val)[30]) (by simp)
+     , memInsert_memInsert_of_ne (b := (toBytes! val)[30]) (by simp)
+     , memInsert_memInsert_of_ne (b := (toBytes! val)[30]) (by simp)
+     , memInsert_memInsert_of_ne (b := (toBytes! val)[30]) (by simp)
+     , memInsert_memInsert_of_ne (b := (toBytes! val)[30]) (by simp)
+     , memInsert_memInsert_of_ne (b := (toBytes! val)[30]) (by simp)
+     , memInsert_memInsert_of_ne (b := (toBytes! val)[30]) (by simp)
+     , memInsert_memInsert_of_ne (b := (toBytes! val)[30]) (by simp)
+     , memInsert_memInsert_of_ne (b := (toBytes! val)[30]) (by simp)
+     , memInsert_memInsert_of_ne (b := (toBytes! val)[30]) (by simp)
+     ]
+  rw [ List.foldr_cons
+     , memInsert_memInsert_of_ne (b := (toBytes! val)[31]) (by simp)
+     , memInsert_memInsert_of_ne (b := (toBytes! val)[31]) (by simp)
+     , memInsert_memInsert_of_ne (b := (toBytes! val)[31]) (by simp)
+     , memInsert_memInsert_of_ne (b := (toBytes! val)[31]) (by simp)
+     , memInsert_memInsert_of_ne (b := (toBytes! val)[31]) (by simp)
+     , memInsert_memInsert_of_ne (b := (toBytes! val)[31]) (by simp)
+     , memInsert_memInsert_of_ne (b := (toBytes! val)[31]) (by simp)
+     , memInsert_memInsert_of_ne (b := (toBytes! val)[31]) (by simp)
+     , memInsert_memInsert_of_ne (b := (toBytes! val)[31]) (by simp)
+     , memInsert_memInsert_of_ne (b := (toBytes! val)[31]) (by simp)
+     , memInsert_memInsert_of_ne (b := (toBytes! val)[31]) (by simp)
+     , memInsert_memInsert_of_ne (b := (toBytes! val)[31]) (by simp)
+     , memInsert_memInsert_of_ne (b := (toBytes! val)[31]) (by simp)
+     , memInsert_memInsert_of_ne (b := (toBytes! val)[31]) (by simp)
+     , memInsert_memInsert_of_ne (b := (toBytes! val)[31]) (by simp)
+     , memInsert_memInsert_of_ne (b := (toBytes! val)[31]) (by simp)
+     , memInsert_memInsert_of_ne (b := (toBytes! val)[31]) (by simp)
+     , memInsert_memInsert_of_ne (b := (toBytes! val)[31]) (by simp)
+     , memInsert_memInsert_of_ne (b := (toBytes! val)[31]) (by simp)
+     , memInsert_memInsert_of_ne (b := (toBytes! val)[31]) (by simp)
+     , memInsert_memInsert_of_ne (b := (toBytes! val)[31]) (by simp)
+     , memInsert_memInsert_of_ne (b := (toBytes! val)[31]) (by simp)
+     , memInsert_memInsert_of_ne (b := (toBytes! val)[31]) (by simp)
+     , memInsert_memInsert_of_ne (b := (toBytes! val)[31]) (by simp)
+     , memInsert_memInsert_of_ne (b := (toBytes! val)[31]) (by simp)
+     , memInsert_memInsert_of_ne (b := (toBytes! val)[31]) (by simp)
+     , memInsert_memInsert_of_ne (b := (toBytes! val)[31]) (by simp)
+     , memInsert_memInsert_of_ne (b := (toBytes! val)[31]) (by simp)
+     , memInsert_memInsert_of_ne (b := (toBytes! val)[31]) (by simp)
+     , memInsert_memInsert_of_ne (b := (toBytes! val)[31]) (by simp)
+     , memInsert_memInsert_of_ne (b := (toBytes! val)[31]) (by simp)
+     ]
+  rw [ ← List.foldr_cons (f := memInsert), ← List.foldr_cons (f := memInsert)
+     , ← List.foldr_cons (f := memInsert), ← List.foldr_cons (f := memInsert)
+     , ← List.foldr_cons (f := memInsert), ← List.foldr_cons (f := memInsert)
+     , ← List.foldr_cons (f := memInsert), ← List.foldr_cons (f := memInsert)
+     , ← List.foldr_cons (f := memInsert), ← List.foldr_cons (f := memInsert)
+     , ← List.foldr_cons (f := memInsert), ← List.foldr_cons (f := memInsert)
+     , ← List.foldr_cons (f := memInsert), ← List.foldr_cons (f := memInsert)
+     , ← List.foldr_cons (f := memInsert), ← List.foldr_cons (f := memInsert)
+     , ← List.foldr_cons (f := memInsert), ← List.foldr_cons (f := memInsert)
+     , ← List.foldr_cons (f := memInsert), ← List.foldr_cons (f := memInsert)
+     , ← List.foldr_cons (f := memInsert), ← List.foldr_cons (f := memInsert)
+     , ← List.foldr_cons (f := memInsert), ← List.foldr_cons (f := memInsert)
+     , ← List.foldr_cons (f := memInsert), ← List.foldr_cons (f := memInsert)
+     , ← List.foldr_cons (f := memInsert), ← List.foldr_cons (f := memInsert)
+     , ← List.foldr_cons (f := memInsert), ← List.foldr_cons (f := memInsert)
+     , ← List.foldr_cons (f := memInsert), ← List.foldr_cons (f := memInsert)
+     ]
+
+lemma foldl_memInsert_reverse {init : Memory} :
+  List.foldl (flip memInsert) init (mkEntries addr val) =
+    List.foldl (flip memInsert) init (mkEntries addr val).reverse := by
+  rw [ List.foldl_reverse, backflip, foldr_memInsert_reverse, List.foldr_reverse, frontflip]
+
+lemma foldr_memInsert_eq_foldl_memInsert {init : Memory} :
+  List.foldr memInsert init (mkEntries addr val) =
+    List.foldl (flip memInsert) init (mkEntries addr val) := by
+  rw [ foldr_memInsert_reverse, List.foldr_reverse, frontflip]
+
+end Memory
+
+section MachineState
+
+variable {addr addr' : UInt256}
+variable {ms : MachineState}
+variable {val val' : UInt256}
+variable {entry : Entry}
+variable {es es' : List Entry}
+
+lemma update_update :
+  (ms.updateMemory addr val).updateMemory addr val' = ms.updateMemory addr val' := by
+  unfold MachineState.updateMemory
+  simp
+
+  rw [ ← mkEntries, ← mkEntries ]
+  rw [ foldr_memInsert_eq_foldl_memInsert ]
+
+  conv => rhs; rw [ foldr_memInsert_eq_foldl_memInsert, foldl_memInsert_reverse ]
+  rw [ mkEntries, mkEntries ]
+
+  rw [ splice_toBytes! val, splice_toBytes! val' ]
+  unfold offsets
+
+  unfold flip
+  simp only [List.map, List.zip, List.zipWith]
+  simp only [Nat.cast_ofNat, Nat.cast_one, Nat.cast_zero]
+
+  rw [ List.foldr_cons, List.foldl_cons, memInsert_memInsert]
+  rw [ List.foldr_cons, List.foldl_cons
+     , memInsert_memInsert_of_ne (by simp), memInsert_memInsert]
+  rw [ List.foldr_cons, List.foldl_cons
+     , memInsert_memInsert_of_ne (by simp), memInsert_memInsert_of_ne (addr := addr + 2) (by simp)
+     , memInsert_memInsert ]
+  rw [ List.foldr_cons, List.foldl_cons
+     , memInsert_memInsert_of_ne (by simp), memInsert_memInsert_of_ne (addr := addr + 3) (by simp)
+     , memInsert_memInsert_of_ne (addr := addr + 3) (by simp)
+     , memInsert_memInsert ]
+  rw [ List.foldr_cons, List.foldl_cons
+     , memInsert_memInsert_of_ne (by simp), memInsert_memInsert_of_ne (addr := addr + 4) (by simp)
+     , memInsert_memInsert_of_ne (addr := addr + 4) (by simp), memInsert_memInsert_of_ne (addr := addr + 4) (by simp)
+     , memInsert_memInsert ]
+  rw [ List.foldr_cons, List.foldl_cons
+     , memInsert_memInsert_of_ne (by simp), memInsert_memInsert_of_ne (addr := addr + 5) (by simp)
+     , memInsert_memInsert_of_ne (addr := addr + 5) (by simp), memInsert_memInsert_of_ne (addr := addr + 5) (by simp)
+     , memInsert_memInsert_of_ne (addr := addr + 5) (by simp)
+     , memInsert_memInsert ]
+  rw [ List.foldr_cons, List.foldl_cons
+     , memInsert_memInsert_of_ne (by simp), memInsert_memInsert_of_ne (addr := addr + 6) (by simp)
+     , memInsert_memInsert_of_ne (addr := addr + 6) (by simp), memInsert_memInsert_of_ne (addr := addr + 6) (by simp)
+     , memInsert_memInsert_of_ne (addr := addr + 6) (by simp), memInsert_memInsert_of_ne (addr := addr + 6) (by simp)
+     , memInsert_memInsert ]
+  rw [ List.foldr_cons, List.foldl_cons
+     , memInsert_memInsert_of_ne (by simp), memInsert_memInsert_of_ne (addr := addr + 7) (by simp)
+     , memInsert_memInsert_of_ne (addr := addr + 7) (by simp), memInsert_memInsert_of_ne (addr := addr + 7) (by simp)
+     , memInsert_memInsert_of_ne (addr := addr + 7) (by simp), memInsert_memInsert_of_ne (addr := addr + 7) (by simp)
+     , memInsert_memInsert_of_ne (addr := addr + 7) (by simp)
+     , memInsert_memInsert ]
+  rw [ List.foldr_cons, List.foldl_cons
+     , memInsert_memInsert_of_ne (by simp), memInsert_memInsert_of_ne (addr := addr + 8) (by simp)
+     , memInsert_memInsert_of_ne (addr := addr + 8) (by simp), memInsert_memInsert_of_ne (addr := addr + 8) (by simp)
+     , memInsert_memInsert_of_ne (addr := addr + 8) (by simp), memInsert_memInsert_of_ne (addr := addr + 8) (by simp)
+     , memInsert_memInsert_of_ne (addr := addr + 8) (by simp), memInsert_memInsert_of_ne (addr := addr + 8) (by simp)
+     , memInsert_memInsert ]
+  rw [ List.foldr_cons, List.foldl_cons
+     , memInsert_memInsert_of_ne (by simp), memInsert_memInsert_of_ne (addr := addr + 9) (by simp)
+     , memInsert_memInsert_of_ne (addr := addr + 9) (by simp), memInsert_memInsert_of_ne (addr := addr + 9) (by simp)
+     , memInsert_memInsert_of_ne (addr := addr + 9) (by simp), memInsert_memInsert_of_ne (addr := addr + 9) (by simp)
+     , memInsert_memInsert_of_ne (addr := addr + 9) (by simp), memInsert_memInsert_of_ne (addr := addr + 9) (by simp)
+     , memInsert_memInsert_of_ne (addr := addr + 9) (by simp)
+     , memInsert_memInsert ]
+  rw [ List.foldr_cons, List.foldl_cons
+     , memInsert_memInsert_of_ne (by simp), memInsert_memInsert_of_ne (addr := addr + 10) (by simp)
+     , memInsert_memInsert_of_ne (addr := addr + 10) (by simp), memInsert_memInsert_of_ne (addr := addr + 10) (by simp)
+     , memInsert_memInsert_of_ne (addr := addr + 10) (by simp), memInsert_memInsert_of_ne (addr := addr + 10) (by simp)
+     , memInsert_memInsert_of_ne (addr := addr + 10) (by simp), memInsert_memInsert_of_ne (addr := addr + 10) (by simp)
+     , memInsert_memInsert_of_ne (addr := addr + 10) (by simp), memInsert_memInsert_of_ne (addr := addr + 10) (by simp)
+     , memInsert_memInsert ]
+  rw [ List.foldr_cons, List.foldl_cons
+     , memInsert_memInsert_of_ne (by simp), memInsert_memInsert_of_ne (addr := addr + 11) (by simp)
+     , memInsert_memInsert_of_ne (addr := addr + 11) (by simp), memInsert_memInsert_of_ne (addr := addr + 11) (by simp)
+     , memInsert_memInsert_of_ne (addr := addr + 11) (by simp), memInsert_memInsert_of_ne (addr := addr + 11) (by simp)
+     , memInsert_memInsert_of_ne (addr := addr + 11) (by simp), memInsert_memInsert_of_ne (addr := addr + 11) (by simp)
+     , memInsert_memInsert_of_ne (addr := addr + 11) (by simp), memInsert_memInsert_of_ne (addr := addr + 11) (by simp)
+     , memInsert_memInsert_of_ne (addr := addr + 11) (by simp)
+     , memInsert_memInsert ]
+  rw [ List.foldr_cons, List.foldl_cons
+     , memInsert_memInsert_of_ne (by simp), memInsert_memInsert_of_ne (addr := addr + 12) (by simp)
+     , memInsert_memInsert_of_ne (addr := addr + 12) (by simp), memInsert_memInsert_of_ne (addr := addr + 12) (by simp)
+     , memInsert_memInsert_of_ne (addr := addr + 12) (by simp), memInsert_memInsert_of_ne (addr := addr + 12) (by simp)
+     , memInsert_memInsert_of_ne (addr := addr + 12) (by simp), memInsert_memInsert_of_ne (addr := addr + 12) (by simp)
+     , memInsert_memInsert_of_ne (addr := addr + 12) (by simp), memInsert_memInsert_of_ne (addr := addr + 12) (by simp)
+     , memInsert_memInsert_of_ne (addr := addr + 12) (by simp), memInsert_memInsert_of_ne (addr := addr + 12) (by simp)
+     , memInsert_memInsert ]
+  rw [ List.foldr_cons, List.foldl_cons
+     , memInsert_memInsert_of_ne (by simp), memInsert_memInsert_of_ne (addr := addr + 13) (by simp)
+     , memInsert_memInsert_of_ne (addr := addr + 13) (by simp), memInsert_memInsert_of_ne (addr := addr + 13) (by simp)
+     , memInsert_memInsert_of_ne (addr := addr + 13) (by simp), memInsert_memInsert_of_ne (addr := addr + 13) (by simp)
+     , memInsert_memInsert_of_ne (addr := addr + 13) (by simp), memInsert_memInsert_of_ne (addr := addr + 13) (by simp)
+     , memInsert_memInsert_of_ne (addr := addr + 13) (by simp), memInsert_memInsert_of_ne (addr := addr + 13) (by simp)
+     , memInsert_memInsert_of_ne (addr := addr + 13) (by simp), memInsert_memInsert_of_ne (addr := addr + 13) (by simp)
+     , memInsert_memInsert_of_ne (addr := addr + 13) (by simp)
+     , memInsert_memInsert ]
+  rw [ List.foldr_cons, List.foldl_cons
+     , memInsert_memInsert_of_ne (by simp), memInsert_memInsert_of_ne (addr := addr + 14) (by simp)
+     , memInsert_memInsert_of_ne (addr := addr + 14) (by simp), memInsert_memInsert_of_ne (addr := addr + 14) (by simp)
+     , memInsert_memInsert_of_ne (addr := addr + 14) (by simp), memInsert_memInsert_of_ne (addr := addr + 14) (by simp)
+     , memInsert_memInsert_of_ne (addr := addr + 14) (by simp), memInsert_memInsert_of_ne (addr := addr + 14) (by simp)
+     , memInsert_memInsert_of_ne (addr := addr + 14) (by simp), memInsert_memInsert_of_ne (addr := addr + 14) (by simp)
+     , memInsert_memInsert_of_ne (addr := addr + 14) (by simp), memInsert_memInsert_of_ne (addr := addr + 14) (by simp)
+     , memInsert_memInsert_of_ne (addr := addr + 14) (by simp), memInsert_memInsert_of_ne (addr := addr + 14) (by simp)
+     , memInsert_memInsert ]
+  rw [ List.foldr_cons, List.foldl_cons
+     , memInsert_memInsert_of_ne (by simp), memInsert_memInsert_of_ne (addr := addr + 15) (by simp)
+     , memInsert_memInsert_of_ne (addr := addr + 15) (by simp), memInsert_memInsert_of_ne (addr := addr + 15) (by simp)
+     , memInsert_memInsert_of_ne (addr := addr + 15) (by simp), memInsert_memInsert_of_ne (addr := addr + 15) (by simp)
+     , memInsert_memInsert_of_ne (addr := addr + 15) (by simp), memInsert_memInsert_of_ne (addr := addr + 15) (by simp)
+     , memInsert_memInsert_of_ne (addr := addr + 15) (by simp), memInsert_memInsert_of_ne (addr := addr + 15) (by simp)
+     , memInsert_memInsert_of_ne (addr := addr + 15) (by simp), memInsert_memInsert_of_ne (addr := addr + 15) (by simp)
+     , memInsert_memInsert_of_ne (addr := addr + 15) (by simp), memInsert_memInsert_of_ne (addr := addr + 15) (by simp)
+     , memInsert_memInsert_of_ne (addr := addr + 15) (by simp)
+     , memInsert_memInsert ]
+  rw [ List.foldr_cons, List.foldl_cons
+     , memInsert_memInsert_of_ne (by simp), memInsert_memInsert_of_ne (addr := addr + 16) (by simp)
+     , memInsert_memInsert_of_ne (addr := addr + 16) (by simp), memInsert_memInsert_of_ne (addr := addr + 16) (by simp)
+     , memInsert_memInsert_of_ne (addr := addr + 16) (by simp), memInsert_memInsert_of_ne (addr := addr + 16) (by simp)
+     , memInsert_memInsert_of_ne (addr := addr + 16) (by simp), memInsert_memInsert_of_ne (addr := addr + 16) (by simp)
+     , memInsert_memInsert_of_ne (addr := addr + 16) (by simp), memInsert_memInsert_of_ne (addr := addr + 16) (by simp)
+     , memInsert_memInsert_of_ne (addr := addr + 16) (by simp), memInsert_memInsert_of_ne (addr := addr + 16) (by simp)
+     , memInsert_memInsert_of_ne (addr := addr + 16) (by simp), memInsert_memInsert_of_ne (addr := addr + 16) (by simp)
+     , memInsert_memInsert_of_ne (addr := addr + 16) (by simp), memInsert_memInsert_of_ne (addr := addr + 16) (by simp)
+     , memInsert_memInsert ]
+  rw [ List.foldr_cons, List.foldl_cons
+     , memInsert_memInsert_of_ne (by simp), memInsert_memInsert_of_ne (addr := addr + 17) (by simp)
+     , memInsert_memInsert_of_ne (addr := addr + 17) (by simp), memInsert_memInsert_of_ne (addr := addr + 17) (by simp)
+     , memInsert_memInsert_of_ne (addr := addr + 17) (by simp), memInsert_memInsert_of_ne (addr := addr + 17) (by simp)
+     , memInsert_memInsert_of_ne (addr := addr + 17) (by simp), memInsert_memInsert_of_ne (addr := addr + 17) (by simp)
+     , memInsert_memInsert_of_ne (addr := addr + 17) (by simp), memInsert_memInsert_of_ne (addr := addr + 17) (by simp)
+     , memInsert_memInsert_of_ne (addr := addr + 17) (by simp), memInsert_memInsert_of_ne (addr := addr + 17) (by simp)
+     , memInsert_memInsert_of_ne (addr := addr + 17) (by simp), memInsert_memInsert_of_ne (addr := addr + 17) (by simp)
+     , memInsert_memInsert_of_ne (addr := addr + 17) (by simp), memInsert_memInsert_of_ne (addr := addr + 17) (by simp)
+     , memInsert_memInsert_of_ne (addr := addr + 17) (by simp)
+     , memInsert_memInsert ]
+  rw [ List.foldr_cons, List.foldl_cons
+     , memInsert_memInsert_of_ne (by simp), memInsert_memInsert_of_ne (addr := addr + 18) (by simp)
+     , memInsert_memInsert_of_ne (addr := addr + 18) (by simp), memInsert_memInsert_of_ne (addr := addr + 18) (by simp)
+     , memInsert_memInsert_of_ne (addr := addr + 18) (by simp), memInsert_memInsert_of_ne (addr := addr + 18) (by simp)
+     , memInsert_memInsert_of_ne (addr := addr + 18) (by simp), memInsert_memInsert_of_ne (addr := addr + 18) (by simp)
+     , memInsert_memInsert_of_ne (addr := addr + 18) (by simp), memInsert_memInsert_of_ne (addr := addr + 18) (by simp)
+     , memInsert_memInsert_of_ne (addr := addr + 18) (by simp), memInsert_memInsert_of_ne (addr := addr + 18) (by simp)
+     , memInsert_memInsert_of_ne (addr := addr + 18) (by simp), memInsert_memInsert_of_ne (addr := addr + 18) (by simp)
+     , memInsert_memInsert_of_ne (addr := addr + 18) (by simp), memInsert_memInsert_of_ne (addr := addr + 18) (by simp)
+     , memInsert_memInsert_of_ne (addr := addr + 18) (by simp), memInsert_memInsert_of_ne (addr := addr + 18) (by simp)
+     , memInsert_memInsert ]
+  rw [ List.foldr_cons, List.foldl_cons
+     , memInsert_memInsert_of_ne (by simp), memInsert_memInsert_of_ne (addr := addr + 19) (by simp)
+     , memInsert_memInsert_of_ne (addr := addr + 19) (by simp), memInsert_memInsert_of_ne (addr := addr + 19) (by simp)
+     , memInsert_memInsert_of_ne (addr := addr + 19) (by simp), memInsert_memInsert_of_ne (addr := addr + 19) (by simp)
+     , memInsert_memInsert_of_ne (addr := addr + 19) (by simp), memInsert_memInsert_of_ne (addr := addr + 19) (by simp)
+     , memInsert_memInsert_of_ne (addr := addr + 19) (by simp), memInsert_memInsert_of_ne (addr := addr + 19) (by simp)
+     , memInsert_memInsert_of_ne (addr := addr + 19) (by simp), memInsert_memInsert_of_ne (addr := addr + 19) (by simp)
+     , memInsert_memInsert_of_ne (addr := addr + 19) (by simp), memInsert_memInsert_of_ne (addr := addr + 19) (by simp)
+     , memInsert_memInsert_of_ne (addr := addr + 19) (by simp), memInsert_memInsert_of_ne (addr := addr + 19) (by simp)
+     , memInsert_memInsert_of_ne (addr := addr + 19) (by simp), memInsert_memInsert_of_ne (addr := addr + 19) (by simp)
+     , memInsert_memInsert_of_ne (addr := addr + 19) (by simp)
+     , memInsert_memInsert ]
+  rw [ List.foldr_cons, List.foldl_cons
+     , memInsert_memInsert_of_ne (by simp), memInsert_memInsert_of_ne (addr := addr + 20) (by simp)
+     , memInsert_memInsert_of_ne (addr := addr + 20) (by simp), memInsert_memInsert_of_ne (addr := addr + 20) (by simp)
+     , memInsert_memInsert_of_ne (addr := addr + 20) (by simp), memInsert_memInsert_of_ne (addr := addr + 20) (by simp)
+     , memInsert_memInsert_of_ne (addr := addr + 20) (by simp), memInsert_memInsert_of_ne (addr := addr + 20) (by simp)
+     , memInsert_memInsert_of_ne (addr := addr + 20) (by simp), memInsert_memInsert_of_ne (addr := addr + 20) (by simp)
+     , memInsert_memInsert_of_ne (addr := addr + 20) (by simp), memInsert_memInsert_of_ne (addr := addr + 20) (by simp)
+     , memInsert_memInsert_of_ne (addr := addr + 20) (by simp), memInsert_memInsert_of_ne (addr := addr + 20) (by simp)
+     , memInsert_memInsert_of_ne (addr := addr + 20) (by simp), memInsert_memInsert_of_ne (addr := addr + 20) (by simp)
+     , memInsert_memInsert_of_ne (addr := addr + 20) (by simp), memInsert_memInsert_of_ne (addr := addr + 20) (by simp)
+     , memInsert_memInsert_of_ne (addr := addr + 20) (by simp), memInsert_memInsert_of_ne (addr := addr + 20) (by simp)
+     , memInsert_memInsert ]
+  rw [ List.foldr_cons, List.foldl_cons
+     , memInsert_memInsert_of_ne (by simp), memInsert_memInsert_of_ne (addr := addr + 21) (by simp)
+     , memInsert_memInsert_of_ne (addr := addr + 21) (by simp), memInsert_memInsert_of_ne (addr := addr + 21) (by simp)
+     , memInsert_memInsert_of_ne (addr := addr + 21) (by simp), memInsert_memInsert_of_ne (addr := addr + 21) (by simp)
+     , memInsert_memInsert_of_ne (addr := addr + 21) (by simp), memInsert_memInsert_of_ne (addr := addr + 21) (by simp)
+     , memInsert_memInsert_of_ne (addr := addr + 21) (by simp), memInsert_memInsert_of_ne (addr := addr + 21) (by simp)
+     , memInsert_memInsert_of_ne (addr := addr + 21) (by simp), memInsert_memInsert_of_ne (addr := addr + 21) (by simp)
+     , memInsert_memInsert_of_ne (addr := addr + 21) (by simp), memInsert_memInsert_of_ne (addr := addr + 21) (by simp)
+     , memInsert_memInsert_of_ne (addr := addr + 21) (by simp), memInsert_memInsert_of_ne (addr := addr + 21) (by simp)
+     , memInsert_memInsert_of_ne (addr := addr + 21) (by simp), memInsert_memInsert_of_ne (addr := addr + 21) (by simp)
+     , memInsert_memInsert_of_ne (addr := addr + 21) (by simp), memInsert_memInsert_of_ne (addr := addr + 21) (by simp)
+     , memInsert_memInsert_of_ne (addr := addr + 21) (by simp)
+     , memInsert_memInsert ]
+  rw [ List.foldr_cons, List.foldl_cons
+     , memInsert_memInsert_of_ne (by simp), memInsert_memInsert_of_ne (addr := addr + 22) (by simp)
+     , memInsert_memInsert_of_ne (addr := addr + 22) (by simp), memInsert_memInsert_of_ne (addr := addr + 22) (by simp)
+     , memInsert_memInsert_of_ne (addr := addr + 22) (by simp), memInsert_memInsert_of_ne (addr := addr + 22) (by simp)
+     , memInsert_memInsert_of_ne (addr := addr + 22) (by simp), memInsert_memInsert_of_ne (addr := addr + 22) (by simp)
+     , memInsert_memInsert_of_ne (addr := addr + 22) (by simp), memInsert_memInsert_of_ne (addr := addr + 22) (by simp)
+     , memInsert_memInsert_of_ne (addr := addr + 22) (by simp), memInsert_memInsert_of_ne (addr := addr + 22) (by simp)
+     , memInsert_memInsert_of_ne (addr := addr + 22) (by simp), memInsert_memInsert_of_ne (addr := addr + 22) (by simp)
+     , memInsert_memInsert_of_ne (addr := addr + 22) (by simp), memInsert_memInsert_of_ne (addr := addr + 22) (by simp)
+     , memInsert_memInsert_of_ne (addr := addr + 22) (by simp), memInsert_memInsert_of_ne (addr := addr + 22) (by simp)
+     , memInsert_memInsert_of_ne (addr := addr + 22) (by simp), memInsert_memInsert_of_ne (addr := addr + 22) (by simp)
+     , memInsert_memInsert_of_ne (addr := addr + 22) (by simp), memInsert_memInsert_of_ne (addr := addr + 22) (by simp)
+     , memInsert_memInsert ]
+  rw [ List.foldr_cons, List.foldl_cons
+     , memInsert_memInsert_of_ne (by simp), memInsert_memInsert_of_ne (addr := addr + 23) (by simp)
+     , memInsert_memInsert_of_ne (addr := addr + 23) (by simp), memInsert_memInsert_of_ne (addr := addr + 23) (by simp)
+     , memInsert_memInsert_of_ne (addr := addr + 23) (by simp), memInsert_memInsert_of_ne (addr := addr + 23) (by simp)
+     , memInsert_memInsert_of_ne (addr := addr + 23) (by simp), memInsert_memInsert_of_ne (addr := addr + 23) (by simp)
+     , memInsert_memInsert_of_ne (addr := addr + 23) (by simp), memInsert_memInsert_of_ne (addr := addr + 23) (by simp)
+     , memInsert_memInsert_of_ne (addr := addr + 23) (by simp), memInsert_memInsert_of_ne (addr := addr + 23) (by simp)
+     , memInsert_memInsert_of_ne (addr := addr + 23) (by simp), memInsert_memInsert_of_ne (addr := addr + 23) (by simp)
+     , memInsert_memInsert_of_ne (addr := addr + 23) (by simp), memInsert_memInsert_of_ne (addr := addr + 23) (by simp)
+     , memInsert_memInsert_of_ne (addr := addr + 23) (by simp), memInsert_memInsert_of_ne (addr := addr + 23) (by simp)
+     , memInsert_memInsert_of_ne (addr := addr + 23) (by simp), memInsert_memInsert_of_ne (addr := addr + 23) (by simp)
+     , memInsert_memInsert_of_ne (addr := addr + 23) (by simp), memInsert_memInsert_of_ne (addr := addr + 23) (by simp)
+     , memInsert_memInsert_of_ne (addr := addr + 23) (by simp)
+     , memInsert_memInsert ]
+  rw [ List.foldr_cons, List.foldl_cons
+     , memInsert_memInsert_of_ne (by simp), memInsert_memInsert_of_ne (addr := addr + 24) (by simp)
+     , memInsert_memInsert_of_ne (addr := addr + 24) (by simp), memInsert_memInsert_of_ne (addr := addr + 24) (by simp)
+     , memInsert_memInsert_of_ne (addr := addr + 24) (by simp), memInsert_memInsert_of_ne (addr := addr + 24) (by simp)
+     , memInsert_memInsert_of_ne (addr := addr + 24) (by simp), memInsert_memInsert_of_ne (addr := addr + 24) (by simp)
+     , memInsert_memInsert_of_ne (addr := addr + 24) (by simp), memInsert_memInsert_of_ne (addr := addr + 24) (by simp)
+     , memInsert_memInsert_of_ne (addr := addr + 24) (by simp), memInsert_memInsert_of_ne (addr := addr + 24) (by simp)
+     , memInsert_memInsert_of_ne (addr := addr + 24) (by simp), memInsert_memInsert_of_ne (addr := addr + 24) (by simp)
+     , memInsert_memInsert_of_ne (addr := addr + 24) (by simp), memInsert_memInsert_of_ne (addr := addr + 24) (by simp)
+     , memInsert_memInsert_of_ne (addr := addr + 24) (by simp), memInsert_memInsert_of_ne (addr := addr + 24) (by simp)
+     , memInsert_memInsert_of_ne (addr := addr + 24) (by simp), memInsert_memInsert_of_ne (addr := addr + 24) (by simp)
+     , memInsert_memInsert_of_ne (addr := addr + 24) (by simp), memInsert_memInsert_of_ne (addr := addr + 24) (by simp)
+     , memInsert_memInsert_of_ne (addr := addr + 24) (by simp), memInsert_memInsert_of_ne (addr := addr + 24) (by simp)
+     , memInsert_memInsert ]
+  rw [ List.foldr_cons, List.foldl_cons
+     , memInsert_memInsert_of_ne (by simp), memInsert_memInsert_of_ne (addr := addr + 25) (by simp)
+     , memInsert_memInsert_of_ne (addr := addr + 25) (by simp), memInsert_memInsert_of_ne (addr := addr + 25) (by simp)
+     , memInsert_memInsert_of_ne (addr := addr + 25) (by simp), memInsert_memInsert_of_ne (addr := addr + 25) (by simp)
+     , memInsert_memInsert_of_ne (addr := addr + 25) (by simp), memInsert_memInsert_of_ne (addr := addr + 25) (by simp)
+     , memInsert_memInsert_of_ne (addr := addr + 25) (by simp), memInsert_memInsert_of_ne (addr := addr + 25) (by simp)
+     , memInsert_memInsert_of_ne (addr := addr + 25) (by simp), memInsert_memInsert_of_ne (addr := addr + 25) (by simp)
+     , memInsert_memInsert_of_ne (addr := addr + 25) (by simp), memInsert_memInsert_of_ne (addr := addr + 25) (by simp)
+     , memInsert_memInsert_of_ne (addr := addr + 25) (by simp), memInsert_memInsert_of_ne (addr := addr + 25) (by simp)
+     , memInsert_memInsert_of_ne (addr := addr + 25) (by simp), memInsert_memInsert_of_ne (addr := addr + 25) (by simp)
+     , memInsert_memInsert_of_ne (addr := addr + 25) (by simp), memInsert_memInsert_of_ne (addr := addr + 25) (by simp)
+     , memInsert_memInsert_of_ne (addr := addr + 25) (by simp), memInsert_memInsert_of_ne (addr := addr + 25) (by simp)
+     , memInsert_memInsert_of_ne (addr := addr + 25) (by simp), memInsert_memInsert_of_ne (addr := addr + 25) (by simp)
+     , memInsert_memInsert_of_ne (addr := addr + 25) (by simp)
+     , memInsert_memInsert ]
+  rw [ List.foldr_cons, List.foldl_cons
+     , memInsert_memInsert_of_ne (by simp), memInsert_memInsert_of_ne (addr := addr + 26) (by simp)
+     , memInsert_memInsert_of_ne (addr := addr + 26) (by simp), memInsert_memInsert_of_ne (addr := addr + 26) (by simp)
+     , memInsert_memInsert_of_ne (addr := addr + 26) (by simp), memInsert_memInsert_of_ne (addr := addr + 26) (by simp)
+     , memInsert_memInsert_of_ne (addr := addr + 26) (by simp), memInsert_memInsert_of_ne (addr := addr + 26) (by simp)
+     , memInsert_memInsert_of_ne (addr := addr + 26) (by simp), memInsert_memInsert_of_ne (addr := addr + 26) (by simp)
+     , memInsert_memInsert_of_ne (addr := addr + 26) (by simp), memInsert_memInsert_of_ne (addr := addr + 26) (by simp)
+     , memInsert_memInsert_of_ne (addr := addr + 26) (by simp), memInsert_memInsert_of_ne (addr := addr + 26) (by simp)
+     , memInsert_memInsert_of_ne (addr := addr + 26) (by simp), memInsert_memInsert_of_ne (addr := addr + 26) (by simp)
+     , memInsert_memInsert_of_ne (addr := addr + 26) (by simp), memInsert_memInsert_of_ne (addr := addr + 26) (by simp)
+     , memInsert_memInsert_of_ne (addr := addr + 26) (by simp), memInsert_memInsert_of_ne (addr := addr + 26) (by simp)
+     , memInsert_memInsert_of_ne (addr := addr + 26) (by simp), memInsert_memInsert_of_ne (addr := addr + 26) (by simp)
+     , memInsert_memInsert_of_ne (addr := addr + 26) (by simp), memInsert_memInsert_of_ne (addr := addr + 26) (by simp)
+     , memInsert_memInsert_of_ne (addr := addr + 26) (by simp), memInsert_memInsert_of_ne (addr := addr + 26) (by simp)
+     , memInsert_memInsert ]
+  rw [ List.foldr_cons, List.foldl_cons
+     , memInsert_memInsert_of_ne (by simp), memInsert_memInsert_of_ne (addr := addr + 27) (by simp)
+     , memInsert_memInsert_of_ne (addr := addr + 27) (by simp), memInsert_memInsert_of_ne (addr := addr + 27) (by simp)
+     , memInsert_memInsert_of_ne (addr := addr + 27) (by simp), memInsert_memInsert_of_ne (addr := addr + 27) (by simp)
+     , memInsert_memInsert_of_ne (addr := addr + 27) (by simp), memInsert_memInsert_of_ne (addr := addr + 27) (by simp)
+     , memInsert_memInsert_of_ne (addr := addr + 27) (by simp), memInsert_memInsert_of_ne (addr := addr + 27) (by simp)
+     , memInsert_memInsert_of_ne (addr := addr + 27) (by simp), memInsert_memInsert_of_ne (addr := addr + 27) (by simp)
+     , memInsert_memInsert_of_ne (addr := addr + 27) (by simp), memInsert_memInsert_of_ne (addr := addr + 27) (by simp)
+     , memInsert_memInsert_of_ne (addr := addr + 27) (by simp), memInsert_memInsert_of_ne (addr := addr + 27) (by simp)
+     , memInsert_memInsert_of_ne (addr := addr + 27) (by simp), memInsert_memInsert_of_ne (addr := addr + 27) (by simp)
+     , memInsert_memInsert_of_ne (addr := addr + 27) (by simp), memInsert_memInsert_of_ne (addr := addr + 27) (by simp)
+     , memInsert_memInsert_of_ne (addr := addr + 27) (by simp), memInsert_memInsert_of_ne (addr := addr + 27) (by simp)
+     , memInsert_memInsert_of_ne (addr := addr + 27) (by simp), memInsert_memInsert_of_ne (addr := addr + 27) (by simp)
+     , memInsert_memInsert_of_ne (addr := addr + 27) (by simp), memInsert_memInsert_of_ne (addr := addr + 27) (by simp)
+     , memInsert_memInsert_of_ne (addr := addr + 27) (by simp)
+     , memInsert_memInsert ]
+  rw [ List.foldr_cons, List.foldl_cons
+     , memInsert_memInsert_of_ne (by simp), memInsert_memInsert_of_ne (addr := addr + 28) (by simp)
+     , memInsert_memInsert_of_ne (addr := addr + 28) (by simp), memInsert_memInsert_of_ne (addr := addr + 28) (by simp)
+     , memInsert_memInsert_of_ne (addr := addr + 28) (by simp), memInsert_memInsert_of_ne (addr := addr + 28) (by simp)
+     , memInsert_memInsert_of_ne (addr := addr + 28) (by simp), memInsert_memInsert_of_ne (addr := addr + 28) (by simp)
+     , memInsert_memInsert_of_ne (addr := addr + 28) (by simp), memInsert_memInsert_of_ne (addr := addr + 28) (by simp)
+     , memInsert_memInsert_of_ne (addr := addr + 28) (by simp), memInsert_memInsert_of_ne (addr := addr + 28) (by simp)
+     , memInsert_memInsert_of_ne (addr := addr + 28) (by simp), memInsert_memInsert_of_ne (addr := addr + 28) (by simp)
+     , memInsert_memInsert_of_ne (addr := addr + 28) (by simp), memInsert_memInsert_of_ne (addr := addr + 28) (by simp)
+     , memInsert_memInsert_of_ne (addr := addr + 28) (by simp), memInsert_memInsert_of_ne (addr := addr + 28) (by simp)
+     , memInsert_memInsert_of_ne (addr := addr + 28) (by simp), memInsert_memInsert_of_ne (addr := addr + 28) (by simp)
+     , memInsert_memInsert_of_ne (addr := addr + 28) (by simp), memInsert_memInsert_of_ne (addr := addr + 28) (by simp)
+     , memInsert_memInsert_of_ne (addr := addr + 28) (by simp), memInsert_memInsert_of_ne (addr := addr + 28) (by simp)
+     , memInsert_memInsert_of_ne (addr := addr + 28) (by simp), memInsert_memInsert_of_ne (addr := addr + 28) (by simp)
+     , memInsert_memInsert_of_ne (addr := addr + 28) (by simp), memInsert_memInsert_of_ne (addr := addr + 28) (by simp)
+     , memInsert_memInsert ]
+  rw [ List.foldr_cons, List.foldl_cons
+     , memInsert_memInsert_of_ne (by simp), memInsert_memInsert_of_ne (addr := addr + 29) (by simp)
+     , memInsert_memInsert_of_ne (addr := addr + 29) (by simp), memInsert_memInsert_of_ne (addr := addr + 29) (by simp)
+     , memInsert_memInsert_of_ne (addr := addr + 29) (by simp), memInsert_memInsert_of_ne (addr := addr + 29) (by simp)
+     , memInsert_memInsert_of_ne (addr := addr + 29) (by simp), memInsert_memInsert_of_ne (addr := addr + 29) (by simp)
+     , memInsert_memInsert_of_ne (addr := addr + 29) (by simp), memInsert_memInsert_of_ne (addr := addr + 29) (by simp)
+     , memInsert_memInsert_of_ne (addr := addr + 29) (by simp), memInsert_memInsert_of_ne (addr := addr + 29) (by simp)
+     , memInsert_memInsert_of_ne (addr := addr + 29) (by simp), memInsert_memInsert_of_ne (addr := addr + 29) (by simp)
+     , memInsert_memInsert_of_ne (addr := addr + 29) (by simp), memInsert_memInsert_of_ne (addr := addr + 29) (by simp)
+     , memInsert_memInsert_of_ne (addr := addr + 29) (by simp), memInsert_memInsert_of_ne (addr := addr + 29) (by simp)
+     , memInsert_memInsert_of_ne (addr := addr + 29) (by simp), memInsert_memInsert_of_ne (addr := addr + 29) (by simp)
+     , memInsert_memInsert_of_ne (addr := addr + 29) (by simp), memInsert_memInsert_of_ne (addr := addr + 29) (by simp)
+     , memInsert_memInsert_of_ne (addr := addr + 29) (by simp), memInsert_memInsert_of_ne (addr := addr + 29) (by simp)
+     , memInsert_memInsert_of_ne (addr := addr + 29) (by simp), memInsert_memInsert_of_ne (addr := addr + 29) (by simp)
+     , memInsert_memInsert_of_ne (addr := addr + 29) (by simp), memInsert_memInsert_of_ne (addr := addr + 29) (by simp)
+     , memInsert_memInsert_of_ne (addr := addr + 29) (by simp)
+     , memInsert_memInsert ]
+  rw [ List.foldr_cons, List.foldl_cons
+     , memInsert_memInsert_of_ne (by simp), memInsert_memInsert_of_ne (addr := addr + 30) (by simp)
+     , memInsert_memInsert_of_ne (addr := addr + 30) (by simp), memInsert_memInsert_of_ne (addr := addr + 30) (by simp)
+     , memInsert_memInsert_of_ne (addr := addr + 30) (by simp), memInsert_memInsert_of_ne (addr := addr + 30) (by simp)
+     , memInsert_memInsert_of_ne (addr := addr + 30) (by simp), memInsert_memInsert_of_ne (addr := addr + 30) (by simp)
+     , memInsert_memInsert_of_ne (addr := addr + 30) (by simp), memInsert_memInsert_of_ne (addr := addr + 30) (by simp)
+     , memInsert_memInsert_of_ne (addr := addr + 30) (by simp), memInsert_memInsert_of_ne (addr := addr + 30) (by simp)
+     , memInsert_memInsert_of_ne (addr := addr + 30) (by simp), memInsert_memInsert_of_ne (addr := addr + 30) (by simp)
+     , memInsert_memInsert_of_ne (addr := addr + 30) (by simp), memInsert_memInsert_of_ne (addr := addr + 30) (by simp)
+     , memInsert_memInsert_of_ne (addr := addr + 30) (by simp), memInsert_memInsert_of_ne (addr := addr + 30) (by simp)
+     , memInsert_memInsert_of_ne (addr := addr + 30) (by simp), memInsert_memInsert_of_ne (addr := addr + 30) (by simp)
+     , memInsert_memInsert_of_ne (addr := addr + 30) (by simp), memInsert_memInsert_of_ne (addr := addr + 30) (by simp)
+     , memInsert_memInsert_of_ne (addr := addr + 30) (by simp), memInsert_memInsert_of_ne (addr := addr + 30) (by simp)
+     , memInsert_memInsert_of_ne (addr := addr + 30) (by simp), memInsert_memInsert_of_ne (addr := addr + 30) (by simp)
+     , memInsert_memInsert_of_ne (addr := addr + 30) (by simp), memInsert_memInsert_of_ne (addr := addr + 30) (by simp)
+     , memInsert_memInsert_of_ne (addr := addr + 30) (by simp), memInsert_memInsert_of_ne (addr := addr + 30) (by simp)
+     , memInsert_memInsert ]
+  rw [ List.foldr_cons, List.foldl_cons
+     , memInsert_memInsert_of_ne (by simp), memInsert_memInsert_of_ne (addr := addr + 31) (by simp)
+     , memInsert_memInsert_of_ne (addr := addr + 31) (by simp), memInsert_memInsert_of_ne (addr := addr + 31) (by simp)
+     , memInsert_memInsert_of_ne (addr := addr + 31) (by simp), memInsert_memInsert_of_ne (addr := addr + 31) (by simp)
+     , memInsert_memInsert_of_ne (addr := addr + 31) (by simp), memInsert_memInsert_of_ne (addr := addr + 31) (by simp)
+     , memInsert_memInsert_of_ne (addr := addr + 31) (by simp), memInsert_memInsert_of_ne (addr := addr + 31) (by simp)
+     , memInsert_memInsert_of_ne (addr := addr + 31) (by simp), memInsert_memInsert_of_ne (addr := addr + 31) (by simp)
+     , memInsert_memInsert_of_ne (addr := addr + 31) (by simp), memInsert_memInsert_of_ne (addr := addr + 31) (by simp)
+     , memInsert_memInsert_of_ne (addr := addr + 31) (by simp), memInsert_memInsert_of_ne (addr := addr + 31) (by simp)
+     , memInsert_memInsert_of_ne (addr := addr + 31) (by simp), memInsert_memInsert_of_ne (addr := addr + 31) (by simp)
+     , memInsert_memInsert_of_ne (addr := addr + 31) (by simp), memInsert_memInsert_of_ne (addr := addr + 31) (by simp)
+     , memInsert_memInsert_of_ne (addr := addr + 31) (by simp), memInsert_memInsert_of_ne (addr := addr + 31) (by simp)
+     , memInsert_memInsert_of_ne (addr := addr + 31) (by simp), memInsert_memInsert_of_ne (addr := addr + 31) (by simp)
+     , memInsert_memInsert_of_ne (addr := addr + 31) (by simp), memInsert_memInsert_of_ne (addr := addr + 31) (by simp)
+     , memInsert_memInsert_of_ne (addr := addr + 31) (by simp), memInsert_memInsert_of_ne (addr := addr + 31) (by simp)
+     , memInsert_memInsert_of_ne (addr := addr + 31) (by simp), memInsert_memInsert_of_ne (addr := addr + 31) (by simp)
+     , memInsert_memInsert_of_ne (addr := addr + 31) (by simp)
+     , memInsert_memInsert ]
+
+  rw [List.foldr_nil]
+  repeat rw [← List.foldl_cons]
+  simp only [List.reverse, List.reverseAux]
+
+lemma update_update_of_ne :
+  (h : ∀ {a}, a ∈ offsets_at addr' → a ∉ offsets_at addr) →
+  (ms.updateMemory addr val).updateMemory addr' val' =
+    (ms.updateMemory addr' val').updateMemory addr val := by
+  intro h
+  unfold MachineState.updateMemory
+  simp
+  apply And.intro
+
+  swap
+  rw [← max_assoc, max_comm addr' addr, max_assoc]
+
+  rw [ ← mkEntries, ← mkEntries ]
+  sorry
+
+lemma lt_toBytes_length_of_mem_offset :
+  ∀ {offset}, (v : UInt256) → (offset ∈ offsets) → offset < (toBytes! v).length := by
+  unfold offsets
+  simp
+
+lemma lookupBytes_nil :
+  ∀ {addr},
+  [].map (ms.memory.lookupByte ∘ (addr + ↑·)) = [] := by
+  simp
+
+lemma lookupBytes_cons :
+  ∀ {addr} {offset : ℕ} {os : List ℕ},
+  (offset :: os).map ((ms.updateMemory addr val).memory.lookupByte ∘ (addr + ↑·)) =
+    (ms.updateMemory addr val).memory.lookupByte (addr + ↑offset)
+    :: os.map ((ms.updateMemory addr val).memory.lookupByte ∘ (addr + ↑·)) := by
+  intro addr offset os
+  exact List.map_cons
+    ((ms.updateMemory addr val).memory.lookupByte ∘ (addr + ↑·))
+    offset
+    os
+
+-- TODO: in newer mathlib
+@[simp] theorem get!_some {α} [Inhabited α] {a : α} : (some a).get! = a := rfl
+
+-- lemma lookupByte_updateMemory :
+--   ∀ {addr},
+--   (ms.updateMemory addr val).memory.lookupByte addr =
+--     (UInt256.toBytes! val)[0] := by
+--   intro addr
+--   unfold MachineState.updateMemory Memory.lookupByte
+--   simp
+--   rw [ List.zipWith_foldl_eq_zip_foldl ]
+--   conv => lhs; rw [splice_toBytes! val]
+--   unfold offsets
+--   simp only [List.map, List.zip, List.zipWith, List.foldl, flip, id]
+--   norm_cast
+--   rw [ Fin.add_zero addr ]
+--   simp
+
+lemma lookupByte_update_of_ne :
+  ∀ {addr addr' : UInt256},
+  (h : addr' ∉ offsets.map (addr + ↑·)) →
+  (ms.updateMemory addr val).memory.lookupByte addr' =
+    ms.memory.lookupByte addr' := by
+  intro addr addr' h
+  unfold MachineState.updateMemory Memory.lookupByte
+  simp
+  rw [splice_toBytes! val]
+  unfold offsets
+  simp [memInsert, List.foldr]
+
+  unfold offsets at h
+  simp at h
+  repeat rw [← ne_eq] at h
+  let ⟨_,_,_,_,_,_,_,_,_,_,_,_,_,_,_,_,_,_,_,_,_,_,_,_,_,_,_,_,_,_,_,_⟩ := h
+
+  rw [ Finmap.lookup_insert_of_ne, Finmap.lookup_insert_of_ne, Finmap.lookup_insert_of_ne
+     , Finmap.lookup_insert_of_ne, Finmap.lookup_insert_of_ne, Finmap.lookup_insert_of_ne
+     , Finmap.lookup_insert_of_ne, Finmap.lookup_insert_of_ne, Finmap.lookup_insert_of_ne
+     , Finmap.lookup_insert_of_ne, Finmap.lookup_insert_of_ne, Finmap.lookup_insert_of_ne
+     , Finmap.lookup_insert_of_ne, Finmap.lookup_insert_of_ne, Finmap.lookup_insert_of_ne
+     , Finmap.lookup_insert_of_ne, Finmap.lookup_insert_of_ne, Finmap.lookup_insert_of_ne
+     , Finmap.lookup_insert_of_ne, Finmap.lookup_insert_of_ne, Finmap.lookup_insert_of_ne
+     , Finmap.lookup_insert_of_ne, Finmap.lookup_insert_of_ne, Finmap.lookup_insert_of_ne
+     , Finmap.lookup_insert_of_ne, Finmap.lookup_insert_of_ne, Finmap.lookup_insert_of_ne
+     , Finmap.lookup_insert_of_ne, Finmap.lookup_insert_of_ne, Finmap.lookup_insert_of_ne
+     , Finmap.lookup_insert_of_ne, Finmap.lookup_insert_of_ne
+     ]
+
+  all_goals assumption
+
+lemma lookupByte_at_offset_update :
+  ∀ {addr} {n}, (mem: n ∈ offsets) →
+  (ms.updateMemory addr val).memory.lookupByte (addr + ↑n) =
+    (UInt256.toBytes! val)[n]'(lt_toBytes_length_of_mem_offset val mem) := by
+  intro addr n mem
+  unfold MachineState.updateMemory Memory.lookupByte
+  simp
+  conv => lhs; rw [splice_toBytes! val]
+  unfold offsets
+  simp only [List.foldr]
+  norm_cast
+  fin_cases mem
+  · rw [ Nat.cast_zero, Fin.add_zero addr ]
+    simp
+  · rw [ Nat.cast_one ]
+    simp
+  all_goals simp only [ Nat.cast_ofNat, memInsert, Fin.isValue, List.getElem_eq_get
+                      , Function.uncurry_apply_pair, add_zero, ne_eq, add_right_eq_self
+                      , Fin.reduceEq, not_false_eq_true, Finmap.lookup_insert_of_ne
+                      , add_right_inj, Finmap.lookup_insert, get!_some
+                      ]
+
+lemma lookupByte_at_offset_update_of_ne {addr addr' : UInt256} :
+  ∀ {n}, (mem: n ∈ offsets) →
+  (h : addr' + ↑n ∉ offsets.map (addr + ↑·)) →
+  (ms.updateMemory addr val).memory.lookupByte (addr' + ↑n) =
+    ms.memory.lookupByte (addr' + ↑n) := by
+  intro n _ _
+  apply lookupByte_update_of_ne (addr' := addr' + ↑n)
+  assumption
+
+lemma lookupWord_update : ∀ {addr},
+  (ms.updateMemory addr val).memory.lookupWord addr = val := by
+  intro addr
+  unfold Memory.lookupWord offsets
+  repeat rw [ lookupBytes_cons, lookupByte_at_offset_update (by simp) ]
+  rw [ List.map_nil
+     , ← splice_toBytes!
+     , fromBytes!_toBytes!
+     ]
+
+lemma lookupWord_update_of_ne {addr addr' : UInt256} :
+  (h : ∀ {n}, (mem: n ∈ offsets) → addr' + ↑n ∉ offsets.map (addr + ↑·)) →
+  (ms.updateMemory addr val).memory.lookupWord addr' = ms.memory.lookupWord addr' := by
+  intro h
+
+  unfold Memory.lookupWord
+
+  rw [ ← List.map_comp_map
+     , Function.comp_apply
+     , ← List.map_comp_map
+     , Function.comp_apply
+     ]
+  simp only [List.map]
+
+  rw [ lookupByte_at_offset_update_of_ne (by simp) (h (by simp))
+     , lookupByte_at_offset_update_of_ne (by simp) (h (by simp))
+     , lookupByte_at_offset_update_of_ne (by simp) (h (by simp))
+     , lookupByte_at_offset_update_of_ne (by simp) (h (by simp))
+     , lookupByte_at_offset_update_of_ne (by simp) (h (by simp))
+     , lookupByte_at_offset_update_of_ne (by simp) (h (by simp))
+     , lookupByte_at_offset_update_of_ne (by simp) (h (by simp))
+     , lookupByte_at_offset_update_of_ne (by simp) (h (by simp))
+     , lookupByte_at_offset_update_of_ne (by simp) (h (by simp))
+     , lookupByte_at_offset_update_of_ne (by simp) (h (by simp))
+     , lookupByte_at_offset_update_of_ne (by simp) (h (by simp))
+     , lookupByte_at_offset_update_of_ne (by simp) (h (by simp))
+     , lookupByte_at_offset_update_of_ne (by simp) (h (by simp))
+     , lookupByte_at_offset_update_of_ne (by simp) (h (by simp))
+     , lookupByte_at_offset_update_of_ne (by simp) (h (by simp))
+     , lookupByte_at_offset_update_of_ne (by simp) (h (by simp))
+     , lookupByte_at_offset_update_of_ne (by simp) (h (by simp))
+     , lookupByte_at_offset_update_of_ne (by simp) (h (by simp))
+     , lookupByte_at_offset_update_of_ne (by simp) (h (by simp))
+     , lookupByte_at_offset_update_of_ne (by simp) (h (by simp))
+     , lookupByte_at_offset_update_of_ne (by simp) (h (by simp))
+     , lookupByte_at_offset_update_of_ne (by simp) (h (by simp))
+     , lookupByte_at_offset_update_of_ne (by simp) (h (by simp))
+     , lookupByte_at_offset_update_of_ne (by simp) (h (by simp))
+     , lookupByte_at_offset_update_of_ne (by simp) (h (by simp))
+     , lookupByte_at_offset_update_of_ne (by simp) (h (by simp))
+     , lookupByte_at_offset_update_of_ne (by simp) (h (by simp))
+     , lookupByte_at_offset_update_of_ne (by simp) (h (by simp))
+     , lookupByte_at_offset_update_of_ne (by simp) (h (by simp))
+     , lookupByte_at_offset_update_of_ne (by simp) (h (by simp))
+     , lookupByte_at_offset_update_of_ne (by simp) (h (by simp))
+     , lookupByte_at_offset_update_of_ne (by simp) (h (by simp))
+     ]
+
+lemma lookupWord_update_of_next {addr : UInt256} :
+  (ms.updateMemory addr val).memory.lookupWord (addr + 32) = ms.memory.lookupWord (addr + 32) := by
+  refine lookupWord_update_of_ne (addr := addr) (addr' := addr + 32) ?h
+  intro n mem
+  fin_cases mem <;> (norm_cast; simp; intro x x_mem)
+  · fin_cases x_mem <;> norm_cast
+  · fin_cases x_mem <;> (norm_cast; try rw [add_assoc]; simp)
+  · fin_cases x_mem <;> (norm_cast; try rw [add_assoc]; simp)
+  · fin_cases x_mem <;> (norm_cast; try rw [add_assoc]; simp)
+  · fin_cases x_mem <;> (norm_cast; try rw [add_assoc]; simp)
+  · fin_cases x_mem <;> (norm_cast; try rw [add_assoc]; simp)
+  · fin_cases x_mem <;> (norm_cast; try rw [add_assoc]; simp)
+  · fin_cases x_mem <;> (norm_cast; try rw [add_assoc]; simp)
+  · fin_cases x_mem <;> (norm_cast; try rw [add_assoc]; simp)
+  · fin_cases x_mem <;> (norm_cast; try rw [add_assoc]; simp)
+  · fin_cases x_mem <;> (norm_cast; try rw [add_assoc]; simp)
+  · fin_cases x_mem <;> (norm_cast; try rw [add_assoc]; simp)
+  · fin_cases x_mem <;> (norm_cast; try rw [add_assoc]; simp)
+  · fin_cases x_mem <;> (norm_cast; try rw [add_assoc]; simp)
+  · fin_cases x_mem <;> (norm_cast; try rw [add_assoc]; simp)
+  · fin_cases x_mem <;> (norm_cast; try rw [add_assoc]; simp)
+  · fin_cases x_mem <;> (norm_cast; try rw [add_assoc]; simp)
+  · fin_cases x_mem <;> (norm_cast; try rw [add_assoc]; simp)
+  · fin_cases x_mem <;> (norm_cast; try rw [add_assoc]; simp)
+  · fin_cases x_mem <;> (norm_cast; try rw [add_assoc]; simp)
+  · fin_cases x_mem <;> (norm_cast; try rw [add_assoc]; simp)
+  · fin_cases x_mem <;> (norm_cast; try rw [add_assoc]; simp)
+  · fin_cases x_mem <;> (norm_cast; try rw [add_assoc]; simp)
+  · fin_cases x_mem <;> (norm_cast; try rw [add_assoc]; simp)
+  · fin_cases x_mem <;> (norm_cast; try rw [add_assoc]; simp)
+  · fin_cases x_mem <;> (norm_cast; try rw [add_assoc]; simp)
+  · fin_cases x_mem <;> (norm_cast; try rw [add_assoc]; simp)
+  · fin_cases x_mem <;> (norm_cast; try rw [add_assoc]; simp)
+  · fin_cases x_mem <;> (norm_cast; try rw [add_assoc]; simp)
+  · fin_cases x_mem <;> (norm_cast; try rw [add_assoc]; simp)
+  · fin_cases x_mem <;> (norm_cast; try rw [add_assoc]; simp)
+  · fin_cases x_mem <;> (norm_cast; try rw [add_assoc]; simp)
+
+lemma addr_no_overlap : ∀ {k : ℕ},
+  (h : k < Memory.maxWords) →
+  addr + (k + 1) * 32 ∉ offsets.map (addr + ↑·) := by
+  intro k h
+  simp
+  intro x x_mem
+  apply ne_of_lt
+  norm_cast
+
+  apply lt_of_le_of_lt (b := Nat.cast 31)
+  · rw [Fin.natCast_le_natCast (by linarith [lt_32_of_mem_offsets x_mem]) (by simp)]
+    apply Nat.le_of_lt_succ
+    exact lt_32_of_mem_offsets x_mem
+  · have succ_k_words_lt_size :
+      (k + 1) * 32 ≤ 115792089237316195423570985008687907853269984665640564039457584007913129639935 := by
+      trans Memory.maxWords * 32
+      · simp
+        rw [Nat.succ_le]
+        exact h
+      · rw [Memory.maxWords]
+        simp
+    rw [Fin.natCast_lt_natCast (by simp) succ_k_words_lt_size]
+    apply Nat.lt_of_lt_of_le
+    · show (31 < 32); simp
+    · linarith
+
+end MachineState
+
+variable {addr addr' p : UInt256}
+variable {evm : EVM}
+variable {val val' : UInt256}
+
+lemma mstore_mstore :
+  mstore (mstore evm p val) p val' = mstore evm p val' := by
+  unfold mstore updateMemory
+  simp
+  exact update_update
+
+lemma mstore_mstore_of_ne :
+  mstore (mstore evm addr val) addr' val' =
+    mstore (mstore evm addr' val') addr val := by
+  unfold mstore updateMemory
+  simp
+  refine update_update_of_ne ?_
+  sorry
+
+lemma lookup_mstore :
+  (mstore evm p val).machine_state.memory.lookupWord p = val := by
+  unfold mstore updateMemory
+  simp
+  rw [lookupWord_update]
+
+lemma lookup_mstore_of_ne {addr addr' : UInt256} :
+  (h : ∀ {n}, (mem: n ∈ offsets) → addr' + ↑n ∉ offsets.map (addr + ↑·)) →
+  (mstore evm addr val).machine_state.memory.lookupWord addr' =
+    evm.machine_state.memory.lookupWord addr' := by
+  intro h
+  unfold mstore updateMemory
+  rw [lookupWord_update_of_ne h]
+
+lemma lookup_mstore_of_next :
+  ∀ {k}, (h : k < Memory.maxWords) →
+  (mstore evm p val).machine_state.memory.lookupWord (p + (k + 1) * 32) =
+    evm.machine_state.memory.lookupWord (p + (k + 1) * 32) := by
+  sorry
+
+section Interval
+
+variable {p : UInt256}
+variable {n : ℕ}
+variable {evm : EVM}
+variable {ms : MachineState}
+variable {val : UInt256}
+
+lemma interval_of_0_eq_nil :
+  mkInterval ms.memory p 0 = [] := by
+  unfold mkInterval words_at
+  simp
+
+lemma interval_eq_lookup_cons : ∀ {n},
+  mkInterval ms.memory p (n + 1) =
+    ms.memory.lookupWord p :: mkInterval ms.memory (p + 32) n := by
+  intro n
+  unfold mkInterval words_at
+  rw [range'_succ p n, List.map_cons]
+
+-- theorem List.range'_succ (s n step) :
+--   List.range' s (n + 1) step = s :: List.range' (s + step) n step := by
+--   simp [List.range', Nat.add_succ, Nat.mul_succ]
+
+-- lemma out_of_range :
+--   ∀ {n}, (h : n ≤ Memory.maxWords) →
+--   mkInterval (mstore evm p val).machine_state.memory (p + 32) n =
+--     mkInterval evm.machine_state.memory (p + 32) n := by
+--   intro n h
+--   induction n generalizing p with
+--   | zero => rw [interval_of_0_eq_nil, interval_of_0_eq_nil]
+--   | succ n' ih =>
+--     have : (2 : UInt256) * 32 = (1 + 1) * 32 := sorry
+--     rw [ interval_eq_lookup_cons
+--        , ← one_mul 32, ← zero_add 1, ← Nat.cast_zero
+--        , lookup_mstore_of_next (p := p) (k := 0) (by simp [Memory.maxWords])
+--        , Nat.cast_zero, zero_add 1, one_mul 32
+--        , add_assoc, ← two_mul 32
+--        , this ]
+--     rw (config := {occs := .pos [1]}) [ ← Nat.cast_one ]
+--     rw [
+--        ]
+
+lemma interval_of_mstore_eq_val_cons :
+  mkInterval (mstore evm p val).machine_state.memory p (n + 1) =
+    val :: mkInterval (mstore evm p val).machine_state.memory (p + 32) n := by
+  rw [ interval_eq_lookup_cons, lookup_mstore ]
+
+lemma interval_of_mstore_eq_val_cons' :
+  ∀ {n}, (h : n < Memory.maxWords) →
+  mkInterval (mstore evm p val).machine_state.memory p (n + 1) =
+    val :: mkInterval evm.machine_state.memory (p + 32) n := by
+  sorry
+  -- intro n h
+  -- induction n generalizing p with
+  -- | zero => admit
+  -- | succ n' =>
+  --   rw [ interval_eq_lookup_cons, lookup_mstore, out_of_range (le_of_lt h) ]
+
+end Interval
 
 end Clear.EVMState
